most of loadorstore logic proven. refactored

src/proof/hashtriemap/hashtriemap.v
@@ -1,753 +1,208 @@
-From iris.program_logic Require Import atomic.
 From iris.bi.lib Require Import atomic.
-From Perennial.program_logic Require Import atomic.
 
+From New.code.hashtriemap Require Import hashtriemap.
 From New.generatedproof.hashtriemap Require Import hashtriemap.
+
+From New.proof Require Import atomic mutex.
+
+From Perennial.algebra Require Import auth_map.
+From Perennial.base_logic.lib Require Import invariants.
+From Perennial.Helpers Require Import NamedProps.
+Import named_props_ascii_notation.
+From Perennial.algebra Require Import ghost_var.
+
 From New.proof.hashtriemap Require Import aux.
-From New.proof.hashtriemap Require Import prelude.
+From New.proof.hashtriemap Require Import paths.
 From New.proof.hashtriemap Require Import model.
-
-From New.proof Require Import sync.
-From New.proof.sync Require Import atomic.
-From Perennial.program_logic Require Import atomic.
-
-From iris.base_logic.lib Require Import invariants.
-From iris.proofmode Require Import proofmode.
-From New.golang.theory Require Import struct.
-
-(* From Perennial.goose_lang.lib Require Import atomic. *)
-From Perennial.algebra Require Import auth_map ghost_var.
-
-Require Import Corelib.Classes.RelationClasses.
-(* From Perennial.goose_lang.lib Require Import atomic. *)
+From New.proof.hashtriemap Require Import hashtriemap_done.
 
 Open Scope Z_scope.
 
 Section proof.
-  Context `{hG: heapGS Σ, !invGS Σ, !ffi_semantics _ _}
+  Context `{hG: heapGS Σ, !ffi_semantics _ _}
     `{!ghost_varG Σ bool}
     `{!ghost_varG Σ (gmap w64 w64)}
     `{!mapG Σ w64 w64}
     `{!mapG Σ Z (gmap w64 w64)}
     `{!globalsGS Σ} {go_ctx: GoContext}.
 
-  Definition map_get `{!IntoVal V} `{!IntoValTyped V t} (v: option V) : V * bool :=
-    (default (default_val V) v, bool_decide (is_Some v)).
-
   #[global] Instance : IsPkgInit hashtriemap := define_is_pkg_init True%I.
   #[global] Instance : GetIsPkgInitWf hashtriemap := build_get_is_pkg_init_wf.
 
-  Lemma next_nibble_eq (key: w64) (path: path) :
-    let h := uint.Z (hash_key key) in
-    let n := w64_word_instance.(word.and)
-                                 (w64_word_instance.(word.sru) (hash_key key)
-                                                      (w64_word_instance.(word.sub) (W64 (sh path)) (W64 4)))
-                                 (W64 15) in
-    length path < 16 → uint.Z n = Z.land (h ≫ (sh path - 4)) 15.
+  Definition orphaned_entry e (key: K) (value: V) n : iProp Σ :=
+    "#Hnode" ∷ e ↦s[hashtriemap.entry :: "node"]□ n ∗
+    "#Hkey" ∷ e ↦s[hashtriemap.entry :: "key"]□ key ∗
+    "#Hvalue" ∷ e ↦s[hashtriemap.entry :: "value"]□ value ∗
+    "Hoverflow" ∷ struct.field_ref_f hashtriemap.entry "overflow" e ↦ᵥ interface.mk (ptrT.id hashtriemap.entry.id) (# null) ∗
+    "#HisEntry" ∷ n ↦s[hashtriemap.node :: "isEntry"]□ true ∗
+    "#Hent" ∷ n ↦s[hashtriemap.node :: "ent"]□ e ∗
+    "#Hind" ∷ n ↦s[hashtriemap.node :: "ind"]□ null.
+  #[global] Transparent orphaned_entry.
+
+  Lemma wp_newEntryNode (key: w64) (value: w64) :
+    {{{ is_pkg_init hashtriemap }}}
+      @! hashtriemap.newEntryNode #key #value
+      {{{ (e: loc) (n: loc), RET (#e); orphaned_entry e key value n }}}.
+  Proof.
+    wp_start.
+    wp_auto.
+    wp_alloc e as "eval".
+    wp_auto.
+    iApply struct_fields_split in "eval".
+    iNamed "eval".
+    simpl.
+    wp_apply wp_Value__Store.
+    iApply fupd_mask_intro; first apply empty_subseteq.
+    iIntros "Hmask".
+    iNext.
+    iFrame "Hoverflow".
+    iIntros "Hoverflow".
+    iMod "Hmask" as "_".
+    iModIntro.
+    wp_auto.
+    wp_alloc n as "n".
+    iApply struct_fields_split in "n".
+    iNamed "n".
+    simpl.
+    iPersist "Hkey".
+    iPersist "Hvalue".
+    iPersist "HisEntry".
+    iPersist "Hent".
+    iPersist "Hind".
+    wp_pure.
+    wp_pure.
+    wp_load.
+    wp_pure.
+    wp_store.
+    iPersist "Hnode".
+    wp_auto.
+    iApply "HΦ".
+    unfold orphaned_entry.
+    iFrame.
+    iFrame "#".
+  Qed.
+
+  (* if you can provide an updated own_path after one program step, then i give you back an entry *)
+  (* Lemma wp_newEntryNode (key: w64) (value: w64) γ path h : *)
+  (*   ∀ Φ, *)
+  (*   is_pkg_init hashtriemap -∗ *)
+  (*   ( *)
+  (*     ⌜uint.Z (hash_key key) = h⌝ ∗ *)
+  (*     ⌜belongs_to_path path h⌝ ∗ *)
+  (*     (|={⊤,∅}=> ∃ rest_map, *)
+  (*        own_path γ.(map_name) 1 path (singleton_map_fn h (<[key:=value]> rest_map)) ∗ *)
+  (*        (∀ e, entry γ 1 e path ={∅,⊤}=∗ Φ #e)) *)
+  (*   ) -∗ *)
+  (*   WP @! hashtriemap.newEntryNode #key #value {{ Φ }}. *)
+  (* (* Lemma wp_newEntryNode (key: w64) (value: w64) γ path h rest_map : *) *)
+  (* (*   {{{ is_pkg_init hashtriemap ∗ *) *)
+  (* (*       ⌜uint.Z (hash_key key) = h⌝ ∗ *) *)
+  (* (*       ⌜belongs_to_path path h⌝ ∗ *) *)
+  (* (*       own_path γ.(map_name) 1 path (singleton_map_fn h (<[key:=value]> rest_map)) *) *)
+  (* (*   }}} *) *)
+  (* (*     @! hashtriemap.newEntryNode #key #value *) *)
+  (* (*     {{{ (e: loc), RET (#e); entry γ 1 e path }}}. *) *)
+  (* Proof. *)
+  (*   wp_start. *)
+  (*   iDestruct "HΦ" as "(Hhash & Hbelongs & Hfupd)". *)
+  (*   wp_auto. *)
+  (*   wp_alloc e as "eval". *)
+  (*   wp_auto. *)
+  (*   iDestruct (typed_pointsto_not_null e 1 ({| *)
+  (*                hashtriemap.entry.node' := null; *)
+  (*                hashtriemap.entry.overflow' := *)
+  (*                  {| atomic.Value.v' := interface.nil |}; *)
+  (*                hashtriemap.entry.key' := key; *)
+  (*                hashtriemap.entry.value' := value *)
+  (*              |}) with "[$eval]") as %enotnull. *)
+  (*   { vm_compute. auto. } *)
+  (*   iApply struct_fields_split in "eval". *)
+  (*   simpl. *)
+  (*   iNamed "eval". *)
+  (*   wp_apply wp_Value__Store. *)
+  (*   iApply fupd_mask_intro; first apply empty_subseteq. *)
+  (*   iIntros "Hmask". *)
+  (*   iNext. *)
+  (*   iFrame "Hoverflow". *)
+  (*   iIntros "Hoverflow". *)
+  (*   iMod "Hmask" as "_". *)
+  (*   iModIntro. *)
+  (*   wp_auto. *)
+  (*   wp_alloc n as "n". *)
+  (*   iApply struct_fields_split in "n". *)
+  (*   simpl. *)
+  (*   iNamed "n". *)
+  (*   iPersist "HisEntry". *)
+  (*   iPersist "Hent". *)
+  (*   iPersist "Hind". *)
+  (*   iPersist "Hkey". *)
+  (*   iPersist "Hvalue". *)
+  (*   (* iDestruct "Hpre" as "[Ha [Hb Hc]]". *) *)
+  (*   iApply fupd_wp. *)
+  (*   (* wp_bind. *) *)
+  (*   (* wp_apply wp_atomic. *) *)
+  (*   (* { apply _. } *) *)
+  (*   iMod "Hfupd". *)
+  (*   iDestruct "Hfupd" as (rest_map) "[Hown_path Hcont]". *)
+  (*   (* iNamed "Hfupd". *) *)
+  (*   (* iDestruct "Hc" as "" *) *)
+  (*   iMod (inv_alloc entryN _ (entry_inv γ 1 (entry γ 1) e path) with "[Hhash Hbelongs Hown_path Hoverflow]") as "Hinv". *)
+  (*   { *)
+  (*     iNext. *)
+  (*     unfold entry_inv. *)
+  (*     rewrite decide_False; [|exact enotnull]. *)
+  (*     unfold entry_step. *)
+  (*     iExists null. *)
+  (*     rewrite /named. *)
+  (*     iFrame "Hhash Hbelongs". *)
+  (*     simpl. *)
+  (*     iSplitL "Hown_path". *)
+  (*     + iExists value. iExists rest_map. *)
+  (*       iFrame "Hown_path". *)
+  (*       iFrame "#". *)
+  (*     + iFrame. *)
+  (*       iNext. *)
+  (*       iFrame. *)
+  (*   } *)
+  (*   iMod ("Hcont" with "[Hinv]") as "HΦ". *)
+  (*   { *)
+  (*     iApply entry_unfold. *)
+  (*     rewrite /entry_F /named. *)
+  (*     iFrame "Hinv". *)
+  (*   } *)
+  (*   iModIntro. *)
+  (*   wp_auto. *)
+  (*   iApply "HΦ". *)
+  (* Qed. *)
+
+  Lemma wp_load_root γ (ht: loc) :
+    ∀ (Φ: val → iProp Σ),
+    is_pkg_init atomic -∗
+    (inv mapN (ht_inv ht γ)) -∗
+    (∀ root : loc,
+       "#Hroot_indirect" :: indirect γ root [] -∗
+       Φ #root)
+    -∗
+    WP interface.type_assert
+      (#
+         (method_callv (ptrT.id atomic.Value.id) "Load"
+            (#(struct.field_ref_f hashtriemap.HashTrieMap "root" ht)))
+         (#()))
+      (#(ptrT.id hashtriemap.indirect.id))
+      {{ v, Φ v }}.
   Proof.
     intros.
-    unfold h.
-    rewrite word.unsigned_and_nowrap.
-    rewrite word.unsigned_sru.
-    - rewrite word.unsigned_sub.
-      f_equiv; [|word].
-      unfold sh.
-      rewrite wrap_small; auto.
-      + f_equiv.
-        unfold sh. word.
-      + replace (uint.Z (W64 (64 - 4 * length path))) with (64 - 4 * length path) by word.
-        replace (uint.Z (W64 4)) with 4 by word.
-        replace (w64_word_instance_ok.(word.wrap) (64 - 4 * length path - 4)) with (64 - 4 * length path - 4) by word.
-        unfold sh in *.
-        have Hx : ((64 - 4 * length path - 4)) ≥ 0 by lia.
-        have Hrng : 0 ≤ uint.Z (hash_key key) < 2^64 by word.
-        split.
-        * apply Z.shiftr_nonneg. lia.
-        * destruct Hrng as [_ Hrng].
-          apply (Z.le_lt_trans _ (uint.Z (hash_key key))); [|exact Hrng].
-          set x := uint.Z (hash_key key).
-          rewrite Z.shiftr_div_pow2; [|word].
-          apply Z.div_le_upper_bound; [word|].
-          set z := 2 ^ (64 - 4 * length path - 4).
-          have Hz : 1 ≤ z.
-          {
-            replace 1 with (2^0) by lia.
-            apply Z.pow_le_mono_r; lia.
-          }
-          replace (z * x) with (x * z) by lia.
-          clear Hx.
-          have Hx : 0 ≤ x by word.
-          have Hy : 1 ≤ z by lia.
-          have : x * 1 ≤ x * z.
-          { apply (Z.mul_le_mono_nonneg_l _ _ _ Hx).
-            exact Hy. }
-          word.
-    - replace (w64_word_instance.(word.sub) (W64 (sh path)) (W64 4)) with (W64 (sh path - 4)) by word.
-      unfold sh.
-      replace (uint.Z (W64 (64 - 4 * length path - 4))) with (64 - 4 * length path - 4) by word.
-      word.
-  Qed.
-
-  Lemma wp_node__entry (n: loc) (e: loc) :
-    {{{ is_pkg_init hashtriemap ∗
-        n ↦s[hashtriemap.node :: "isEntry"]□ true ∗
-        n ↦s[hashtriemap.node :: "ent"]□ e }}}
-      n @ (ptrT.id hashtriemap.node.id) @ "entry" #()
-      {{{ RET #e; True }}}.
-  Proof.
-    wp_start as "(His_entry & Hent)".
-    wp_auto.
-    wp_finish.
-  Qed.
-
-  Lemma wp_node__indirect (n: loc) (i: loc) :
-    {{{ is_pkg_init hashtriemap ∗
-        n ↦s[hashtriemap.node :: "isEntry"]□ false ∗
-        n ↦s[hashtriemap.node :: "ind"]□ i }}}
-      n @ (ptrT.id hashtriemap.node.id) @ "indirect" #()
-      {{{ RET #i; True }}}.
-  Proof.
-    wp_start as "(His_entry & Hind)".
-    wp_auto.
-    wp_finish.
-  Qed.
-
-  Lemma own_path_lookup γ q path h f :
-    h ∈ path_to_domain path →
-    own_path γ q path f -∗
-    ptsto_mut γ h q (f h) ∗ (ptsto_mut γ h q (f h) -∗ own_path γ q path f).
-  Proof.
-    iIntros (Hdom) "Hpath".
-    iDestruct (big_sepL_elem_of_acc with "Hpath") as "[Hptsto Hpath_close]"; [exact Hdom|].
-    iFrame "Hptsto Hpath_close".
-  Qed.
-
-  (* precondition: returns value, true if k is in kvs *)
-  Lemma wp_entry__lookup (ht: loc) (e: loc) (key: K) (γ: ghost_names) (path: path) :
-    ∀ (Φ: val → iProp Σ),
-    is_pkg_init hashtriemap -∗
-    "Hpre" :: (
-      "#His_map" :: is_hashtriemap γ ht ∗
-      "Hentry" :: entry γ (1/2)%Qp e path ∗
-      "Hau" :: ht_au γ (λ m, Φ (ht_load_ret m key)) ∗
-      "%Hbelongs" :: ⌜belongs_to_path path (uint.Z (hash_key key))⌝
-    ) -∗
-    WP e @ (ptrT.id hashtriemap.entry.id) @ "lookup" #key {{ Φ }}.
-  Proof.
-    intros.
-    set h := (uint.Z (hash_key key)).
-    iIntros.
-    iNamed.
-    iNamed "Hpre".
-    wp_method_call. wp_call.
-
-    wp_auto.
-
-    iAssert (
-        ∃ e,
-          "e" :: e_ptr ↦ e ∗
-          "#Hentry" :: entry γ (1 / 2) e path
-      )%I with "[$e $Hentry]" as "Hloop".
-    clear e.
-
-    wp_for "Hloop".
-
-    wp_if_destruct.
-    {
-      iApply fupd_wp.
-      iEval (rewrite entry_unfold /entry_F) in "Hentry".
-      iNamed "His_map".
-      iInv "His_map" as (rooti hm user_map) "(>? & >? & >? & #Hroot_indirect & >? & >?)" "Hclose_map".
-      iNamed.
-      iInv "Hentry_inv" as "HEI" "Hclose_entry".
-      unfold entry_inv.
-      iEval (simpl) in "HEI".
-      iMod "HEI".
-      iNamed.
-      iMod (fupd_mask_subseteq (⊤ ∖ ↑mapN ∖ ↑indN ∖ ↑entryN)) as "Hclose_au_mask"; [set_solver|].
-      iMod "Hau" as (m) "[Hown Hclose_au]".
-
-      iDestruct (ghost_var_agree with "Hown Huser_map") as %Heq.
-      subst m.
-
-      have Hdom : h ∈ path_to_domain path.
-      {
-        rewrite list_elem_of_filter.
-        split; [exact Hbelongs|].
-        apply full_domain_elem.
-      }
-
-      iDestruct (own_path_lookup _ _ _ h with "Hown_empty") as "[Hptsto Hptsto_close]"; [exact Hdom|].
-      iDestruct (map_valid with "Hauth_map Hptsto") as %Hlookup.
-      iDestruct ("Hptsto_close" with "Hptsto") as "Hown_empty".
-
-      have Hnone : user_map !! key = None.
-      {
-        rewrite Hflat.
-        rewrite (Hbuckets _ _ _ Hlookup); done.
-      }
-
-      iNamed.
-
-      iMod ("Hclose_au" with "[$]") as "HΦ".
-      iMod "Hclose_au_mask" as "_".
-      iMod ("Hclose_entry" with "[Hown_empty]") as "_"; [iNext; done|].
-      iMod ("Hclose_map" with "[$Hauth_map $Hown_root $Hroot_indirect $Hown //]") as "_".
-      iApply fupd_mask_intro; [set_solver|].
-      iIntros "_".
-      wp_alloc ret as "ret".
-      wp_auto.
-      simpl.
-      unfold ht_load_ret.
-      iEval (rewrite Hnone; simpl) in "HΦ".
-      iApply "HΦ".
-    }
-
-    iApply fupd_wp.
-    rewrite entry_unfold /entry_F.
-    iNamed.
-
-    iInv "Hentry_inv" as "HEI" "Hclose_entry".
-    unfold entry_inv.
-    destruct (decide (e = null)); [exfalso; auto|].
-    iDestruct "HEI" as (next) "(>? & HEI)".
-    iNamed.
-
-    iNamed "Hentry_step".
-
-    destruct (bool_decide (k = key)) eqn:Heq_key.
-
-    - apply bool_decide_eq_true in Heq_key.
-      replace h0 with h by (unfold h; subst; reflexivity).
-
-      iNamed "His_map".
-      iInv "His_map" as (rooti hm user_map) "(>? & >? & >? & #Hroot_indirect & >? & >?)" "Hclose_map".
-      iNamed.
-      iMod (fupd_mask_subseteq (⊤ ∖ ↑mapN ∖ ↑indN ∖ ↑entryN)) as "Hclose_au_mask"; [set_solver|].
-      iMod "Hau" as (m) "[Hown Hclose_au]".
-
-      (* linearization point *)
-
-      iDestruct (ghost_var_agree with "Hown Huser_map") as %Heq.
-      subst m.
-
-      have Hdom : h ∈ path_to_domain path.
-      {
-        rewrite list_elem_of_filter.
-        split; [exact Hbelongs|].
-        apply full_domain_elem.
-      }
-
-      iDestruct (own_path_lookup _ _ _ h with "Hown_path") as "[Hptsto Hptsto_close]"; [exact Hdom|].
-      iDestruct (map_valid with "Hauth_map Hptsto") as %Hlookup.
-      iDestruct ("Hptsto_close" with "Hptsto") as "Hown_path".
-
-      have Hsome : user_map !! key = Some v.
-      {
-        subst k.
-        rewrite Hflat.
-        rewrite (Hbuckets _ _ _ Hlookup); try done.
-        unfold singleton_map_fn.
-        rewrite decide_True; [|done].
-        rewrite lookup_insert.
-        rewrite decide_True; done.
-      }
-
-      iNamed.
-
-      iMod ("Hclose_au" with "[$]") as "HΦ".
-
-      iMod "Hclose_au_mask" as "_".
-      iMod ("Hclose_map" with "[$Hauth_map $Hown_root $Hroot_indirect $Hown //]") as "_".
-      iMod ("Hclose_entry" with "[$Hown_path $HEI]") as "_".
-      {
-        iFrame "#".
-        iPureIntro. subst k. done.
-      }
-
-      iApply fupd_mask_intro; [set_solver|].
-      iIntros "_".
-      wp_auto.
-      wp_if_destruct; [|exfalso; auto].
-
-      wp_for_post.
-
-      unfold ht_load_ret.
-
-      iEval (rewrite Hsome; simpl) in "HΦ".
-      iApply "HΦ".
-
-    - apply bool_decide_eq_false in Heq_key.
-
-      iMod ("Hclose_entry" with "[$Hown_path $HEI]") as "_"; [iFrame "#"; iPureIntro; done|].
-
-      iApply fupd_mask_intro; [set_solver|].
-      iIntros "_".
-
-      wp_auto.
-
-      wp_if_destruct; [exfalso; auto|].
-      clear Heq_key.
-      wp_apply wp_Value__Load.
-
-      iInv "Hentry_inv" as "HEI" "Hclose_entry".
-      unfold entry_inv.
-      destruct (decide (e = null)); [exfalso; auto|].
-      clear next.
-      iDestruct "HEI" as (next) "(>? & HEI)".
-      iNamed.
-
-      iApply fupd_mask_intro; [set_solver|].
-      iIntros "Hmask".
-      iNext.
-
-      iNamed "HEI".
-      iFrame "Hown_next".
-      iIntros "Hown_next".
-
-      iMod "Hmask" as "_".
-      iMod ("Hclose_entry" with "[$Hentry_step $Hown_next $Hnext_entry]") as "_".
-
-      iApply fupd_mask_intro; [set_solver|].
-      iIntros "_".
-
-      wp_apply wp_interface_type_assert; [auto|].
-
-      wp_for_post.
-      iFrame.
-      iFrame "Hnext_entry".
-  Qed.
-
-  Lemma wp_hashInt (key: w64) (seed: w64) :
-    {{{ is_pkg_init hashtriemap }}}
-      @! hashtriemap.hashInt #key #seed
-      {{{ (a: w64), RET (#a); ⌜a = hash_key key⌝ }}}.
-  Proof. Admitted.
-
-  Lemma wp_newIndirectNode (γ: ghost_names) (parent: loc) (path: list Z) (hm: hash_map) :
-    {{{ is_pkg_init hashtriemap }}}
-      @! hashtriemap.newIndirectNode #parent
-      {{{ (ind: loc), RET (#ind);
-          indirect γ ind path }}}.
-  Proof.
-    wp_start as "Hpre".
-    wp_auto.
-    rename i_ptr into ind_ptr.
-    iRename "i" into "ind".
-
-    wp_apply (wp_slice_make2 (V:=atomic.Value.t)).
-    { unfold hashtriemap.nChildren. word. }
-    iIntros (children) "(Hchildren & _)".
-    wp_auto.
-    wp_alloc ind_struct as "ind_struct".
-    wp_auto.
-
-    set (children_vs := replicate (sint.nat (W64 hashtriemap.nChildren))
-                                  atomic.into_val_typed_Value.(default_val atomic.Value.t)).
-
-    iAssert (
-        ∃ (vs: list atomic.Value.t) (idx i: w64),
-          "Hvs" :: children ↦* vs ∗
-          "i" :: i_ptr ↦ i ∗
-          "idx" :: idx_ptr ↦ idx ∗
-          "%Hi_idx" :: ⌜sint.Z i >= sint.Z idx⌝ ∗
-          "%Hi_bound" :: ⌜uint.Z i <= hashtriemap.nChildren⌝ ∗
-          "%Hlen" :: ⌜length vs = Z.to_nat hashtriemap.nChildren⌝ ∗
-          "%Hprefix" :: ⌜∀ (j: nat), j ≥ 0 → j < uint.Z i →
-                                     ∃ av, vs !! j = Some av ∧
-                                           av = atomic.Value.mk (interface.mk (ptrT.id hashtriemap.node.id) (# null))⌝ ∗
-          "%Hsuffix" :: ⌜∀ (j: nat), j >= uint.Z i → j < length vs → vs !! j = children_vs !! j⌝
-      )%I with "[$Hchildren $i $idx]" as "IH".
-    {
-      iNamed.
-      unfold hashtriemap.nChildren.
-      iPureIntro.
-      simpl.
-      split_and!; auto; try word.
-      iIntros (j Hj Hj2).
-      exfalso.
-      word.
-    }
-
-    wp_for "IH".
-
-    iDestruct (own_slice_len_keep with "Hvs") as "(Hvs & %Hlen_slice & _)".
-
-    wp_if_destruct.
-    2: {
-      wp_alloc node as "node".
-
-      iApply struct_fields_split in "ind_struct".
-      iNamed "ind_struct".
-      iApply struct_fields_split in "node".
-      iNamed "node".
-      simpl.
-      wp_auto.
-
-      iAssert (
-          indirect γ ind_struct path
-        )%I with "[Hvs Hnode Hdead Hmu Hparent Hchildren HisEntry Hent Hind]" as "Hinv".
-      {
-        (* TODO: whatever this invariant ends up being, need to prove it here with M=∅ *)
-        admit.
-      }
-
-      iApply "HΦ".
-      iFrame "Hinv".
-    }
-
-    wp_pure.
-    { split; word. }
-
-    have Hlookup_vs : (vs !! sint.nat i = Some (atomic.into_val_typed_Value.(default_val atomic.Value.t))).
-    {
-      have Hidx_lt : uint.nat i < length vs.
-      { rewrite Hlen. word. }
-
-      have Hsuffix_i : vs !! uint.nat i = children_vs !! uint.nat i.
-      { apply Hsuffix; [lia|exact Hidx_lt]. }
-
-      have Hsuit : sint.nat i = uint.nat i.
-      { word. }
-
-      rewrite Hsuit.
-      rewrite Hsuffix_i.
-      rewrite lookup_replicate_2; auto.
-      word.
-    }
-
-    wp_apply (wp_load_slice_elem with "[$Hvs]"); auto.
-    { word. }
-
-    iIntros "Hvs".
-
-    wp_auto.
-
-    wp_pure.
-    { split; cbn; word. }
-
-    wp_auto.
-
-    iDestruct ((own_slice_elem_acc) with "[$Hvs]") as "[Helem Hcont]"; eauto.
-    { word. }
-
-    iAssert (own_Value (slice.elem_ref_f children atomic.Value i) 1 interface.nil)%I
-      with "[Helem]" as "Helem".
-    {
-      auto.
-    }
-
-    wp_apply wp_Value__Store.
-
-    iApply fupd_mask_intro.
-    { set_solver. }
-    iIntros "Hmask".
-    iNext.
-    iFrame "Helem".
-    iIntros "Helem".
-    iMod "Hmask".
-    iClear "Hmask".
-    iApply fupd_mask_intro.
-    {set_solver. }
-    iIntros "_".
-    wp_auto.
-
-    iDestruct ("Hcont" with "Helem") as "Hvs".
-
-    wp_for_post.
-
-    iFrame "HΦ ind ind_struct".
-
-    iFrame.
-
-    iSplit.
-    { word. }
-
-    iSplit.
-    { word. }
-    iSplit.
-    {
-      iPureIntro.
-      rewrite length_insert.
-      exact Hlen.
-    }
-    iSplit.
-    - iPureIntro. intros j Hj_ge Hj_lt.
-
-      have Hj_lte : j ≤ uint.Z i.
-      { word. }
-      clear Hj_lt.
-
-      apply Z_le_lt_eq_dec in Hj_lte.
-      destruct Hj_lte as [Hlt | Heq].
-
-      + (* j < i *)
-        specialize (Hprefix j) as Hprefix.
-        specialize (Hprefix Hj_ge Hlt).
-        destruct Hprefix as (av & Hlookup & Hav).
-        exists av.
-        split; auto.
-
-        rewrite list_lookup_insert_ne; auto.
-        word.
-      + (* j = i *)
-        exists {| atomic.Value.v' := interface.mk (ptrT.id hashtriemap.node.id) (# null) |}.
-        split; auto.
-        rewrite list_lookup_insert.
-        have Hbool : (sint.nat i = j ∧ (sint.nat i < length vs)%nat)%nat.
-        { word. }
-        by destruct (decide (sint.nat i = j ∧ (sint.nat i < length vs)%nat)) as [H|H];
-        [reflexivity | exfalso; exact (H Hbool)].
-    - iPureIntro. intros j Hj_ge Hj_lt.
-
-      have Hj_ge_i1_nat : (j ≥ uint.nat i + 1)%nat.
-      { word. }
-      have Hj_ge_i_Z : (j >= uint.Z i).
-      { word. }
-      have Hj_ge_i1_Z : (j >= uint.Z i + 1).
-      { word. }
-      have Hj_lt_len : (j < length vs).
-      { rewrite length_insert in Hj_lt. word. }
-
-      specialize (Hsuffix j) as Hsuffix.
-      specialize (Hsuffix Hj_ge_i_Z Hj_lt_len).
-      rewrite list_lookup_insert_ne; auto.
-      word.
-  Admitted.            (* only admitted because of the ind invariant needing proof *)
-
-  Lemma wp_HashTrieMap__initSlow (ht: loc) (γ: ghost_names) (* P {Htimeless: ∀ m, Timeless (P m)} *) :
-    {{{ is_pkg_init hashtriemap ∗ is_pkg_init atomic ∗ is_pkg_init sync ∗
-        hashtriemap_init ht γ }}}
-      ht @ (ptrT.id hashtriemap.HashTrieMap.id) @ "initSlow" #()
-      {{{ RET #();
-          hashtriemap_init ht γ (* P *) ∗ is_hashtriemap γ ht (* P *) }}}.
-  Proof.
-    wp_start as "Hpre".
-    iDestruct "Hpre" as "(#Hinit & #Hmu)".
-
-    wp_apply wp_with_defer as "%defer defer"; simpl subst.
-    wp_auto.
-
-    wp_apply (wp_Mutex__Lock with "[$Hmu]").
-    iIntros "(Hown_mutex&Hmu_inv)".
-    wp_auto.
-
-    wp_apply wp_Uint32__Load.
-    iInv "Hinit" as (b) "(>Hinited & >Hinit_tok & #Hstatus_done)" "Hclose".
-    iApply fupd_mask_intro.
-    { set_solver. }
-    iIntros "Hmask".
-    iNext.
-    iFrame.
-
-    iIntros "Hinited".
-
-    iDestruct (persistently_elim with "Hstatus_done") as "#Hstatus_done'".
-    iClear "Hstatus_done".
-    iRename "Hstatus_done'" into "Hstatus_done".
-
-    destruct b; simpl in *.
-    {
-      iMod "Hmask".
-      iClear "Hmask".
-      iMod ("Hclose" with "[Hinit_tok Hinited Hstatus_done]") as "_".
-      { iNext; iFrame; iFrame "Hinited Hstatus_done". }
-      iApply fupd_mask_intro.
-      { set_solver. }
-      iIntros "_".
-      wp_auto.
-
-      wp_apply (wp_Mutex__Unlock with "[$Hmu $Hown_mutex $Hmu_inv]").
-
-      wp_finish.
-      iFrame "Hinit Hmu".
-      iExact "Hstatus_done".
-    }
-
-    iDestruct "Hmu_inv" as (b) "Hmu_inv".
-    destruct b.
-    {
-      iDestruct (ghost_var_agree with "Hmu_inv Hinit_tok") as %Heq.
-      inversion Heq.
-    }
-
-    iMod "Hmask".
-    iClear "Hmask".
-    iMod ("Hclose" with "[Hinit_tok Hinited Hstatus_done]") as "_".
-    { iNext; iFrame; iFrame "Hstatus_done Hinited". }
-    iApply fupd_mask_intro.
-    { set_solver. }
-    iIntros "_".
-    wp_auto.
-
-    (* TODO: have lemma to initialize empty_map, and give the ptsto_mut part to newIndirectNode and the auth_map used for constructing ht_inv below *)
-    wp_apply (wp_newIndirectNode γ null [] ∅).
-    iIntros (root_node_ptr) "root_node".
-    wp_auto.
-
-    iFrame.
-    wp_apply wp_Value__Store.
-
-    iInv "Hinit" as (b) "(>Hinited & >Hinit_tok & _)" "Hclose".
-    iApply fupd_mask_intro; [set_solver|].
-    iIntros "Hmask".
-    iNext.
-    iFrame.
-    iExists interface.nil.
-
-    iDestruct "Hmu_inv" as "(Hinit_tok2 & Hseed & Hroot)".
-    iDestruct (ghost_var_agree with "Hinit_tok Hinit_tok2") as %Heq.
-    subst b.
-
-    iFrame.
-
-    iIntros "Hroot".
-    iMod "Hmask".
-    iClear "Hmask".
-    iMod ("Hclose" with "[Hinit_tok Hinited Hstatus_done]") as "_".
-    {
-      iNext.
-      iFrame.
-      iFrame "Hstatus_done Hinited".
-    }
-
-    iApply fupd_mask_intro.
-    { set_solver. }
-    iIntros "_".
-    wp_auto.
-
-    iDestruct "Hseed" as (seed) "Hseed".
-
-    wp_apply (wp_store_ty with "Hseed").
-    Unshelve.
-    2: { eapply into_val_typed_w64. }
-
-    iIntros "Hseed".
-    iPersist "Hseed".
-
-    wp_auto.
-    wp_apply wp_Uint32__Store.
-
-    iInv "Hinit" as (b) "(>Hinited & >Hinit_tok & _)" "Hclose".
-    iApply fupd_mask_intro.
-    { set_solver. }
-    iIntros "Hmask".
-    iNext.
-    iFrame.
-    iIntros "Hinited".
-    iMod "Hmask".
-    iClear "Hmask".
-    destruct b.
-    {
-      iDestruct (ghost_var_agree with "Hinit_tok Hinit_tok2") as %Heq.
-      exfalso. congruence.
-    }
-
-    iMod (ghost_var_update_halves true with "Hinit_tok Hinit_tok2") as "(Htok1 & Htok2)".
-
-    iAssert (ht_inv ht γ)%I (* with "[$]" *) as "Hhtinv".
-    {
-      admit.
-    }
-
-    iMod (invariants.inv_alloc mapN _ (
-              "Hinv" :: ht_inv ht γ
-            ) with "[$Hhtinv]") as "#His_map".
-
-    iMod ("Hclose" with "[Htok1 Hinited His_map]") as "_".
-    { iNext. iFrame. iFrame "Hinited". unfold init_status_done. iFrame "His_map Hseed". }
-    iApply fupd_mask_intro.
-    {set_solver. }
-    iIntros "_".
-    wp_auto.
-
-    iAssert (init_mu_inv ht γ)%I with "[Htok2]" as "Hmu_inv_true".
-    { simpl. iExists true. iFrame "Htok2". }
-
-    wp_apply (wp_Mutex__Unlock with "[$Hmu $Hown_mutex $Hmu_inv_true]").
-    wp_finish.
-    iFrame.
-    iFrame "His_map Hmu Hinit".
-  Admitted.
-
-  (*precondition: either inited is 0 and we call initSlow, or its 1 and we already have the initialization requirements*)
-  Lemma wp_HashTrieMap__initHT (ht: loc) (γ: ghost_names) (* P {Htimeless: ∀ m, Timeless (P m)} *) :
-    {{{ is_pkg_init hashtriemap ∗ is_pkg_init atomic ∗ is_pkg_init sync ∗
-        hashtriemap_init ht γ (* P *) }}}
-      ht @ (ptrT.id hashtriemap.HashTrieMap.id) @ "initHT" #()
-      {{{ RET #();
-          hashtriemap_init ht γ (* P *) ∗ is_hashtriemap γ ht (* P *) }}}.
-  Proof.
-    wp_start as "Hpre".
-    iDestruct "Hpre" as "(#Hinit & #Hmu)".
-
-    wp_auto.
-
-    wp_apply wp_Uint32__Load.
-    iInv "Hinit" as "Hinit2" "Hclose".
-    iApply fupd_mask_intro.
-    { set_solver. }
-    iIntros "Hmask".
-    iNext.
-    iDestruct "Hinit2" as (b) "(Hinited & Hinit_tok & #Hstatus_done)".
-    iFrame.
-    iIntros "Hinited".
-    iMod "Hmask".
-    iClear "Hmask".
-    iMod ("Hclose" with "[Hinit_tok Hinited Hstatus_done]") as "_".
-    { iNext. iFrame. iFrame "Hstatus_done". }
-    iApply fupd_mask_intro.
-    { set_solver. }
-    iIntros "_".
-    wp_auto.
-
-    wp_if_destruct.
-    - wp_apply (wp_HashTrieMap__initSlow).
-      { iFrame. iFrame "Hinit Hmu". }
-      iIntros.
-      wp_finish.
-    - wp_finish.
-      iFrame.
-      destruct b; simpl.
-      + iFrame "Hinit Hmu".
-        iExact "Hstatus_done".
-      + exfalso. congruence.
-  Qed.
-
-  (* dont actually need the is_hashtriemap precondition for any of the lemmas because initHT gives it to us *)
-  Lemma wp_HashTrieMap__Load (ht: loc) (key: w64) (γ: ghost_names) :
-    ∀ (Φ: val → iProp Σ),
-    (is_pkg_init hashtriemap ∗ is_pkg_init atomic ∗ is_pkg_init sync ∗
-     "Hinit" :: hashtriemap_init ht γ ∗
-     "Hau" :: ht_au γ (λ m, Φ (ht_load_ret m key))) -∗
-    WP ht @ (ptrT.id hashtriemap.HashTrieMap.id) @ "Load" #key {{ Φ }}.
-  Proof.
-    iIntros (Φ) "(#? & #? & #? & Hpre)".
-    iNamed "Hpre".
-
-    wp_method_call. wp_call.
-
-    wp_auto.
-
-    wp_apply (wp_HashTrieMap__initHT with "[$]").
-    iIntros "(_ & His_map)".
-    iNamed "His_map".
-    wp_auto.
-
-    wp_apply wp_hashInt.
-    iIntros (hash) "%Hhash".
-
-    wp_auto.
-
-    wp_apply wp_Value__Load.
+    iIntros "#?".
+    iIntros "#His_map".
+    iIntros "HΦ".
+
+    wp_apply (wp_Value__Load with "[$]").
     iInv "His_map" as "Hhtinv" "Hclose".
     iApply fupd_mask_intro.
     { set_solver. }
     iIntros "Hmask".
     iNext.
     iNamed "Hhtinv".
-    iEval (unfold ht_inv) in "Hinv".
-    iNamed "Hinv".
     iFrame "Hown_root".
     iIntros "Hown_root".
     iMod "Hmask".
@@ -760,43 +215,115 @@ Section proof.
     { set_solver. }
     iIntros "_".
 
-    clear Hflat.
-    clear Hbuckets.
-    clear hm. clear user_map.
-
     wp_apply wp_interface_type_assert.
     { auto. }
+    iApply "HΦ".
+    iExact "Hroot_indirect".
+  Qed.
+
+  Lemma wp_HashTrieMap__LoadOrStore (ht: loc) (key: K) (value: V) (γ: ghost_names) :
+    ∀ (Φ: val → iProp Σ),
+    (is_pkg_init hashtriemap ∗ is_pkg_init atomic ∗ is_pkg_init sync) -∗
+    ("Hinit" :: hashtriemap_init ht γ ∗
+    "Hau" ::
+      AU <{ ∃∃ m : gmap K V, own_ht_map γ m }>
+      @ ht_au_mask, ∅
+                    <{ ∀∀ new_m load_res new_v,
+                         ⌜ (new_m, load_res, new_v) = match m !! key with
+                                               | Some old_v => (m, true, old_v)
+                                               | None => (<[key := value]> m, false, value)
+                                               end ⌝ ∗
+                         own_ht_map γ new_m, COMM Φ (#new_v, #load_res)%V }>)
+                      -∗
+                    WP ht @ (ptrT.id hashtriemap.HashTrieMap.id) @ "LoadOrStore" #key #value {{ Φ }}.
+  Proof.
+    wp_start.
+    iNamed "HΦ".
+
+    wp_apply wp_with_defer as "%defer defer"; simpl subst.
+    wp_auto.
+
+    wp_apply (wp_HashTrieMap__initHT with "[$]").
+    iIntros.
+    iNamed.
+    iNamed "His_map".
+    wp_auto.
+
+    wp_apply wp_hashInt.
+    iIntros (hash) "%Hhash".
+
+    wp_auto.
+    iPersist "hash".
+    iPersist "key".
+    iPersist "value".
+
+    iAssert (
+        (* ∃ (HIP: bool), *)
+        (*   if HIP *)
+        (*   then *)
+        (*     ∃ nodeptr children_slice next_nibble path cur, *)
+        (*       "slot" ∷ slot_ptr ↦ slice.elem_ref_f children_slice atomic.Value next_nibble ∗ *)
+        (*       "n" ∷ n_ptr ↦ nodeptr ∗ *)
+        (*       "Hcur" ∷ i_ptr ↦ cur ∗ *)
+        (*       "Hhash_shift" ∷ hashShift_ptr ↦ w64_word_instance.(word.sub) (W64 (sh path)) (W64 4) *)
+        (*   else *)
+            ∃ slot n i shift,
+              "slot" :: slot_ptr ↦ slot ∗
+              "n" :: n_ptr ↦ n ∗
+              "i" ∷ i_ptr ↦ i ∗
+              "hashShift" ∷ hashShift_ptr ↦ shift
+      )%I with "[$slot $n $i $hashShift]" as "Houter_loop_inv".
+
+    wp_for "Houter_loop_inv".
+
+    wp_bind (
+        interface.type_assert
+          (#
+             (method_callv (ptrT.id atomic.Value.id) "Load"
+                (#(struct.field_ref_f hashtriemap.HashTrieMap "root" ht)))
+             (#()))
+          (#(ptrT.id hashtriemap.indirect.id))
+          ).
+
+    iApply (wp_load_root with "[# $] [//]").
+    iIntros.
+    iNamed.
+    wp_auto.
 
     set h := uint.Z (hash_key key).
 
-    iAssert (∃ (path: path) (shift: w64) (cur: loc),
+    iAssert (∃ (path: path) (shift: w64) (cur: loc) (HIP: bool) (sl: loc) (n: loc),
+                "slot" ∷ slot_ptr ↦ sl ∗
+                "n" ∷ n_ptr ↦ n ∗
                 "Hcur" :: i_ptr ↦ cur ∗
                 "Hhash_shift" :: hashShift_ptr ↦ shift ∗
                 "#Hi_indirect" :: indirect γ cur path ∗
                 "%Hshift" :: ⌜shift = sh path⌝ ∗
                 "%Hpath_len" :: ⌜length path < 16⌝ ∗
-                "%Hkey_path" :: ⌜belongs_to_path path h⌝
-            )%I with ("[$Hroot_indirect $hashShift $i]") as "Hloop_inv".
+                "%Hkey_path" :: ⌜belongs_to_path path h⌝ ∗
+                "haveInsertPoint" :: haveInsertPoint_ptr ↦ HIP ∗ (* HIP actually doesnt matter *)
+                "%HIP" :: ⌜shift ≠ 0⌝
+            )%I with ("[$Hroot_indirect $hashShift $i $haveInsertPoint $slot $n]") as "Hloop_inv".
     {
-      repeat iSplit; eauto.
-      iPureIntro.
+      repeat iSplit; eauto; iPureIntro; eauto.
       unfold belongs_to_path, sh, path_to_prefix.
       simpl.
       rewrite Z.shiftr_div_pow2; try word.
     }
-    iClear "Hroot_indirect".
 
     wp_for "Hloop_inv".
+
+    simpl.
 
     iEval (rewrite indirect_unfold /indirect_F) in "Hi_indirect".
     iNamed "Hi_indirect".
 
     wp_if_destruct.
     {
-      wp_apply wp_panic.
-      iPureIntro.
-      unfold sh in e.
-      word.
+      simpl in *.
+      exfalso.
+      apply HIP0.
+      exact e.
     }
 
     iDestruct (own_slice_len with "Hchildren_slice") as "(%Hlen_children_16 & _)".
@@ -865,7 +392,6 @@ Section proof.
       - apply full_domain_elem.
     }
 
-    unfold ht_au.
     wp_apply wp_Value__Load.
     iInv "His_map" as "Hhtinv" "Hclose_ht".
     iInv "Hind_inv" as "HI" "Hclose_ind".
@@ -883,6 +409,7 @@ Section proof.
 
     iNamed "Hhtinv".
     iNamed "Hinv".
+    iNamedSuffix "Hinv" "2".
 
     iDestruct (big_sepL_lookup_acc with "Hchildren") as "[Hchild Hchildren_close]".
     { exact Hv. }
@@ -895,39 +422,19 @@ Section proof.
     unfold ht_load_ret.
     iEval (unfold childP) in "Hchild".
 
-    unfold own_path.
+    (* unfold own_path. *)
 
     destruct (decide (nodeptr = null)).
     {
       iMod "Hmask" as "_".
 
-      iMod (fupd_mask_subseteq ht_au_mask) as "Hclose_au_mask".
-      {
-        unfold ht_au_mask.
-        apply subseteq_difference_l.
-        set_solver.
-      }
-
-      iMod "Hau" as (m) "[Hown Hclose_au]". (* linearization point *)
-      iDestruct (ghost_var_agree with "Huser_map Hown") as %meq.
-      subst m.
-
-      iDestruct (big_sepL_elem_of_acc with "Hchild") as "[Hptsto Hptsto_close]".
-      { exact Hdom. }
-      iDestruct (map_valid with "Hauth_map Hptsto") as %Hlookup.
-      iDestruct ("Hptsto_close" with "Hptsto") as "Hchild".
-
       iDestruct ("Hchildren_close" with "[Hown_child Hchild]") as "Hchildren".
-      { iExists nodeptr. iFrame. unfold childP.
-        destruct (decide (nodeptr = null)).
-        - iFrame.
-        - contradiction n0.
-      }
+      { iExists nodeptr. iFrame. unfold childP. rewrite decide_True; [iFrame|exact e]. }
 
-      iMod ("Hclose_au" with "Hown") as "HΦ".
-      iMod "Hclose_au_mask" as "_".
       iMod ("Hclose_ind" with "Hchildren") as "_".
-      iMod ("Hclose_ht" with "[$Hauth_map $Hown_root $Hroot_indirect $Huser_map //]") as "_".
+      iMod ("Hclose_ht" with "[$Hown_root2 $Hauth_map $Huser_map]") as "_".
+      { iFrame "#". done. }
+      clear hm user_map Hflat2 Hbuckets2 Hbuckets_rev2.
 
       iApply fupd_mask_intro.
       { set_solver. }
@@ -941,29 +448,312 @@ Section proof.
       2: { symmetry. rewrite (bool_decide_eq_true (nodeptr = null)). exact e. }
 
       wp_auto.
-      wp_bind.
-      wp_alloc d_ptr as "d_ptr".
-      wp_auto.
       wp_for_post.
 
-      have Hnone : (user_map !! key = None).
-      {
-        subst user_map.
+      wp_apply wp_Mutex__Lock.
+      { iFrame "#". }
+
+      iIntros "(Hown_mutex & Hx)".
+      iNamed "Hx".
+      iEval (unfold childrenP) in "Hmu_inv".
+      iNamed "Hmu_inv".
+
+      wp_auto.
+
+      wp_apply (wp_Value__Load with "[$]").
+      iApply fupd_mask_intro; first apply empty_subseteq.
+      iIntros "Hmask".
+      iNext.
+
+      iDestruct (big_sepL_lookup_acc with "Hchildren") as "[Hchild Hchildren_close]".
+      { exact Hv. }
+      iNamed "Hchild".
+      iExists (interface.mk (ptrT.id hashtriemap.node.id) (# nodeptr0)).
+      replace (W64 (sint.nat next_nibble)) with next_nibble by word.
+      iFrame "Hown_child".
+      iIntros "Hown_child".
+
+      iMod "Hmask" as "_".
+      iModIntro.
+
+      wp_apply wp_interface_type_assert; [auto|].
+      wp_if_destruct.
+      - wp_apply wp_Bool__Load.
+        iApply fupd_mask_intro; first apply empty_subseteq.
+        iIntros "Hmask".
+        iFrame "Hdead".
+        iIntros "Hdead".
+        iMod "Hmask" as "_".
+        iApply fupd_mask_intro; first set_solver.
+        iIntros "_".
+        simpl.
+
+        wp_if_destruct.
+        {
+          iDestruct ("Hchildren_close" with "[$Hchild $Hown_child]") as "Hchildren".
+          wp_apply (wp_Mutex__Unlock with "[$Hind_mutex $Hdead $Hchildren $Hown_mutex]").
+          wp_for_post.
+          iFrame.
+        }
+        wp_for_post.
+
+        iFrame.
+        iEval (unfold childP) in "Hchild".
+        iSimpl in "Hchild".
+
+        wp_apply wp_newEntryNode.
+        iIntros (e n2) "orphaned".
+        unfold orphaned_entry.
+        iNamedSuffix "orphaned" "_o".
+
+        wp_auto.
+        wp_apply wp_Value__Store.
+
+        iClear "Hroot_indirect".
+        iClear "Hroot_indirect2".
+        clear rooti.
+
+        iInv "His_map" as (rooti hm user_map) "(>? & >? & >? & Hroot_indirect & >? & >? & >?)" "Hclose_map".
+        iInv "Hind_inv" as "Hind" "Hclose_ind_inv".
+        iEval (unfold childrenP) in "Hind".
+        iNamed.
+        iMod (fupd_mask_subseteq ht_au_mask) as "Hau_close_mask".
+        { unfold ht_au_mask; apply subseteq_difference_l; set_solver. }
+
+        iDestruct (big_sepL_elem_of_acc with "Hchild") as "[Hptsto Hptsto_close]".
+        { exact Hdom. }
+        iDestruct (map_valid with "Hauth_map Hptsto") as %Hlookup.
+        iDestruct ("Hptsto_close" with "Hptsto") as "Hchild".
+
+        iMod "Hau" as (user_map2) "(Huser_map2 & [_ Hau_close])".
+
+        iDestruct (ghost_var_agree with "Huser_map Huser_map2") as %Heq.
+        subst user_map2.
+        iMod (ghost_var_update_halves (<[key:=value]> user_map) with "Huser_map Huser_map2") as "[Huser_map Huser_map2]".
+
+        iDestruct (big_sepL_lookup_acc with "Hind") as "[Hchild2 Hchildren_close2]"; [exact Hv|].
+        iDestruct "Hchild2" as (nodeptr2) "[>Hown_child2 Hchild2]".
+        iNamedSuffix "Hown_child2" "2".
+        replace (W64 (sint.nat next_nibble)) with next_nibble by word.
+        iDestruct (own_Value_agree with "Hown_child Hown_child2") as %Heq.
+        inversion Heq.
+        clear Heq.
+        apply (inj to_val) in H0.
+        subst nodeptr2.
+        iEval (unfold childP) in "Hchild2".
+        iSimpl in "Hchild2".
+        iMod "Hchild2".
+        iNamedSuffix "Hchild2" "2".
+
+        iMod (own_path_update_key key value with "Hauth_map [Hchild Hchild2]") as "[Hauth_map Hchild]".
+        { exact Hkey_path. }
+        { iCombine "Hchild Hchild2" as "Hchild". iExact "Hchild". }
+
+        iNamed.
+        iEval (rewrite decide_True) in "Hctx".
+        unfold empty_map_fn.
+        subst h.
+        set h := uint.Z (hash_key key).
+
+        have Hnone : (user_map !! key = None).
+        {
+          subst user_map.
+          unfold empty_map_fn in Hlookup.
+          have Hflat : flatten hm !! key = (∅ : gmap K V) !! key.
+          { apply (Hbuckets h ∅ key); [exact Hlookup|reflexivity]. }
+          rewrite Hflat.
+          rewrite lookup_empty.
+          done.
+        }
+
+        iMod ("Hau_close" with "[$Huser_map2]") as "HΦ".
+        {
+          rewrite Hnone.
+          auto.
+        }
+
+        iMod "Hau_close_mask" as "_".
+        iApply (fupd_mask_intro); first apply empty_subseteq.
+        iIntros "Hmask".
+        iNext.
+        iNamed.
+
+        change (λ h' : Z, if decide (h' = h) then <[key:=value]> ∅ else ∅)
+          with (singleton_map_fn h (<[key:=value]> ∅)).
+
+        iCombine "Hown_child Hown_child2" as "Hown_child".
+        iFrame.
+        iIntros "[Hown_child Hown_child2]".
+        iDestruct (field_pointsto_not_null with "HisEntry_o") as %Hnn.
+        { simpl. done. }
+        { auto. }
+        iDestruct (field_pointsto_not_null with "Hnode_o") as %Hen.
+        { simpl. done. }
+        { auto. }
+
+        iDestruct "Hpath" as "[Hown_path Hown_path2]".
+        iDestruct "Hoverflow_o" as "[Hoverflow Hoverflow2]".
+
+        (* TODO: make entry invariant instance of as_fractional because what is even this *)
+        iMod (inv_alloc entryN _ (entry_inv γ (1/2) (entry γ (1/2)) e path) with "[Hoverflow Hown_path]") as "Hinv".
+        {
+          iNext.
+          unfold entry_inv.
+          rewrite decide_False; [|exact Hen].
+          (* unfold entry_step. *)
+          iExists null.
+          rewrite /named.
+          iFrame.
+          iFrame "#".
+          simpl.
+          iPureIntro; done.
+        }
+        iMod (inv_alloc entryN _ (entry_inv γ (1/2) (entry γ (1/2)) e path) with "[Hoverflow2 Hown_path2]") as "Hinv2".
+        {
+          iNext.
+          unfold entry_inv.
+          rewrite decide_False; [|exact Hen].
+          (* unfold entry_step. *)
+          iExists null.
+          rewrite /named.
+          iFrame.
+          iFrame "#".
+          simpl.
+          iPureIntro; done.
+        }
+
+        iDestruct ("Hchildren_close2" with "[$Hown_child2 Hinv]") as "Hchildren2".
+        {
+          rewrite /named.
+          unfold childP.
+          rewrite decide_False; [|exact Hnn].
+          iFrame "#".
+          iFrame "#".
+          iSplit; [iPureIntro; exact Hen|].
+          iApply entry_unfold.
+          unfold entry_F.
+          iFrame.
+        }
+        iMod "Hmask" as "_".
+
+        iMod ("Hclose_ind_inv" with "[Hchildren2]") as "_".
+        {
+          iNext.
+          unfold childrenP.
+          iFrame "Hchildren2".
+        }
+
         unfold empty_map_fn in Hlookup.
-        have Hflat : flatten hm !! key = (∅ : gmap K V) !! key.
-        { apply (Hbuckets h ∅ key); [exact Hlookup|reflexivity]. }
-        rewrite Hflat.
-        rewrite lookup_empty.
-        done.
-      }
-      iEval (rewrite Hnone; simpl) in "HΦ".
-      iApply "HΦ".
+        replace (uint.Z (hash_key key)) with h in * by reflexivity.
+
+        iMod ("Hclose_map" with "[Huser_map Hctx Hown_root Hroot_indirect]") as "_".
+        {
+          iNext.
+          rewrite /named.
+          unfold ht_inv.
+          iExists rooti.
+          iExists (<[h:=<[key:=value]> ∅]> hm).
+          rewrite /named.
+          iFrame.
+          iFrame "#".
+          iPureIntro.
+          set hm' := <[h := <[key:=value]> ∅]> hm.
+          set um' := <[key:=value]> user_map.
+
+          assert (Hum' : (um' = flatten hm')).
+          {
+            subst um' hm'.
+            symmetry.
+            subst user_map.
+            apply (flatten_update_update hm h key value ∅ ).
+            - exact Hlookup.
+            - reflexivity.
+            - intros.
+              eapply Hbuckets_rev.
+              + exact H.
+              + exact H0.
+         }
+
+         split; [exact Hum'|].
+          split.
+          {
+            intros h0 sub k Hhm' Hhash.
+            rewrite -Hum'.
+            subst um' hm'.
+            destruct (decide (h0 = h)) as [->|Hneq].
+            - rewrite lookup_insert in Hhm'.
+              rewrite decide_True in Hhm'; [|reflexivity].
+              inversion Hhm'; subst sub; clear Hhm'.
+              destruct (decide (k = key)) as [->|Hk].
+              + rewrite lookup_insert. rewrite lookup_insert.
+                rewrite decide_True; [|reflexivity].
+                rewrite decide_True; [|reflexivity].
+                done.
+              + rewrite lookup_insert_ne; [|done].
+                have Hnone_k : user_map !! k = None.
+                { rewrite Hflat.
+                  have Hflatk : flatten hm !! k = (∅ : gmap K V) !! k
+                                                    by apply (Hbuckets h ∅ k Hlookup Hhash).
+                  rewrite Hflatk lookup_empty. done.
+                }
+                rewrite Hnone_k.
+                rewrite lookup_insert_ne; [|done].
+                rewrite lookup_empty. done.
+            - rewrite lookup_insert_ne in Hhm'; [|done].
+              have Hsub : hm !! h0 = Some sub := Hhm'.
+              destruct (decide (k = key)) as [->|Hk].
+              + exfalso. apply Hneq.
+                subst h. rewrite Hhash.
+                done.
+              + rewrite lookup_insert_ne; [|done].
+                rewrite Hflat.
+                eapply Hbuckets; eauto.
+          }
+          {
+            intros.
+            subst hm'.
+            destruct (decide (h0 = h)) as [->|Hneq].
+            - rewrite lookup_insert in H.
+              rewrite decide_True in H; [|done].
+              inversion H; subst sub; clear H.
+              destruct (decide (k = key)) as [->|Hk].
+              + done.
+              + rewrite lookup_insert_ne in H0; [|done].
+                rewrite lookup_empty in H0. discriminate.
+            - rewrite lookup_insert_ne in H; [|done].
+              eapply Hbuckets_rev; eauto.
+          }
+        }
+
+        iModIntro.
+
+        wp_auto.
+
+        iDestruct ("Hchildren_close" with "[Hown_child Hnode_o Hinv2]") as "Hchildren".
+        {
+          iFrame.
+          unfold childP.
+          rewrite decide_False; [|exact Hnn].
+          iFrame "#".
+          iExists e.
+          iSplit; [done|].
+          iFrame "#".
+          iApply entry_unfold.
+          unfold entry_F.
+          iFrame "Hinv2".
+        }
+
+        wp_apply (wp_Mutex__Unlock with "[$Hind_mutex $Hown_mutex $Hdead $Hchildren]").
+
+        iApply "HΦ".
+
+      - shelve.
     }
 
     iDestruct "Hchild" as (is_entry) "(#Hnodeis_entry & #Hchild)".
     destruct is_entry.
     {
-      iDestruct "Hchild" as (ent) "(#Hent & #Hind_null & #Hentry)".
+      iDestruct "Hchild" as (ent) "(%Henotnull & #Hent & #Hind_null & #Hentry)".
       iMod "Hmask" as "_".
 
       iEval (rewrite entry_unfold /entry_F) in "Hentry".
@@ -977,15 +767,16 @@ Section proof.
       }
 
       iDestruct ("Hchildren_close" with "[Hown_child]") as "Hchildren".
-      { iExists nodeptr. iFrame. unfold childP.
+      {
+        iExists nodeptr. iFrame. unfold childP.
         destruct (decide (nodeptr = null)).
-        - contradiction n0.
-        - iExists true. iFrame "#". rewrite entry_unfold /entry_F. iFrame "#".
+        - exfalso. apply n2. exact e.
+        - iExists true. iFrame "#". rewrite entry_unfold /entry_F. iFrame "#". done.
       }
 
       iMod "Hclose_au_mask" as "_".
       iMod ("Hclose_ind" with "[$Hchildren]") as "_".
-      iMod ("Hclose_ht" with "[$Hauth_map $Hown_root $Hroot_indirect $Huser_map //]") as "_".
+      iMod ("Hclose_ht" with "[$Hauth_map $Hown_root2 $Hroot_indirect2 $Huser_map //]") as "_".
 
       iApply fupd_mask_intro.
       { set_solver. }
@@ -994,53 +785,100 @@ Section proof.
       wp_apply wp_interface_type_assert.
       { auto. }
       replace (bool_decide (nodeptr = null)) with false.
-      2: { symmetry. rewrite (bool_decide_eq_false (nodeptr = null)). exact n0. }
+      2: { symmetry. rewrite (bool_decide_eq_false (nodeptr = null)). exact n2. }
 
       wp_auto.
 
-      wp_apply wp_node__entry; [iFrame "Hnodeis_entry Hent"|].
+      wp_apply (wp_node__entry with "[# $]").
       wp_apply wp_entry__lookup.
-      iFrame "His_map Hseed".
+      iFrame "#".
       rewrite /named.
       repeat iSplit; eauto.
       {
-        rewrite entry_unfold /entry_F.
-        iFrame "Hentry_inv".
+        rewrite entry_unfold /entry_F /named.
+
+        iFrame "#".
       }
-      unfold ht_au.
-      iMod "Hau".
-      iApply fupd_mask_intro.
-      { apply empty_subseteq. }
-
+      iAuIntro.
+      rewrite /atomic_acc.
+      iMod "Hau" as (m) "[Hown Hclose_au]".
+      (* iApply aupd_aacc in "Hau". *)
+      iApply fupd_mask_intro; first set_solver.
       iIntros "_".
-      iDestruct "Hau" as (m) "[Huser_own Hclose_au]".
-      iFrame "Huser_own".
-      iIntros "Huser_own".
+      iFrame "Hown".
+      iSplit; iIntros "Hown".
+      {
+        iMod ("Hclose_au" with "Hown") as "Hau".
+        iApply fupd_mask_intro; first set_solver.
+        iIntros "_".
+        iFrame.
+      }
+      destruct (bool_decide (is_Some (m !! key))) eqn:His_some.
+      - (* apply bool_decide_eq_true in His_some. *)
 
-      iDestruct ("Hclose_au" with "Huser_own") as "Hau".
-      iMod "Hau".
+        apply bool_decide_eq_true_1 in His_some.
+        destruct His_some as [old_v Hv_lookup].
 
-      iApply fupd_mask_intro.
-      { set_solver. }
-      iIntros "_".
+        iDestruct "Hclose_au" as "(_ & Hclose_au)".
+        iSpecialize ("Hclose_au" $! m true old_v).
 
-      wp_auto.
-      wp_for_post.
-      iFrame.
+        iMod ("Hclose_au" with "[$Hown]") as "HΦ".
+        {
+          iPureIntro.
+          destruct (m !! key) eqn:Hlookup; simpl.
+          - inversion Hv_lookup.
+            subst. reflexivity.
+          - apply None_ne_Some in Hv_lookup.
+            contradiction.
+        }
+
+        iApply fupd_mask_intro; first set_solver.
+        iIntros "_".
+        iFrame.
+
+        wp_auto.
+        replace (bool_decide (is_Some (m !! key))) with true.
+        2: {
+          symmetry. apply bool_decide_eq_true.
+          auto.
+        }
+        wp_auto.
+        wp_for_post.
+        wp_for_post.
+        replace (default (W64 0) (m !! key)) with old_v.
+        + iExact "HΦ".
+        + rewrite Hv_lookup.
+          simpl.
+          reflexivity.
+      - apply bool_decide_eq_false in His_some.
+        iMod ("Hclose_au" with "Hown") as "Hau".
+        iApply fupd_mask_intro; first set_solver.
+        iIntros "_".
+        iFrame.
+
+        wp_auto.
+        replace (bool_decide (is_Some (m !! key))) with false by (symmetry; apply bool_decide_eq_false; exact His_some).
+        wp_auto.
+
+        wp_for_post.
+
+        clear His_some m.
+
+        shelve.
     }
     iDestruct "Hchild" as (ind) "(%Hnext_path_len & #Hent_null & #Hind & #Hindirect)".
 
     iDestruct ("Hchildren_close" with "[Hown_child]") as "Hchildren".
     { iExists nodeptr. iFrame. unfold childP.
       destruct (decide (nodeptr = null)).
-      - contradiction n0.
+      - exfalso. congruence.
       - iExists false. iFrame "#".
         iPureIntro. exact Hnext_path_len.
     }
 
     iMod "Hmask" as "_".
     iMod ("Hclose_ind" with "Hchildren") as "_".
-    iMod ("Hclose_ht" with "[$Hauth_map $Hown_root $Hroot_indirect $Huser_map //]") as "_".
+    iMod ("Hclose_ht" with "[$Hauth_map $Hown_root2 $Hroot_indirect2 $Huser_map //]") as "_".
 
     iApply fupd_mask_intro.
     { set_solver. }
@@ -1050,20 +888,22 @@ Section proof.
     { auto. }
 
     replace (bool_decide (nodeptr = null)) with false.
-    2: { symmetry. rewrite (bool_decide_eq_false (nodeptr = null)). exact n0. }
+    2: { symmetry. rewrite (bool_decide_eq_false (nodeptr = null)). congruence. }
 
     wp_auto.
     wp_apply (wp_node__indirect with "[$]").
     wp_for_post.
     iFrame.
     iFrame "#".
-    iPureIntro.
+    simpl.
+
+    (* iFrame "slot". *)
 
     set next := Z.of_nat (sint.nat next_nibble).
     set next_path := (path ++ [next]).
 
     have Hlen : length next_path = (length path + 1)%nat by
-                                         rewrite app_length /=.
+                                     rewrite app_length /=.
 
     have Hz : uint.Z next_nibble = Z.land (h ≫ (sh path - 4)) 15.
     {
@@ -1072,23 +912,152 @@ Section proof.
       - auto.
     }
 
-    split_and!; auto.
-    - rewrite sh_snoc. unfold sh. word.
-    - apply (next_nibble_extend path h next); try done.
-      + unfold h.
-        pose proof (word.unsigned_range (hash_key key)) as [H0 _].
-        exact H0.
-      + unfold next.
-        rewrite Z2Nat.id; [|word].
-        rewrite <- Z2Nat.id with (n:=sint.Z next_nibble) by word.
-        word.
-  Qed.
+    iFrame.
+    iPureIntro.
 
-  Lemma wp_HashTrieMap__LoadOrStore (ht: loc) (key: w64) (value: w64) :
-    {{{ is_pkg_init hashtriemap }}}
-      ht @ (ptrT.id hashtriemap.HashTrieMap.id) @ "LoadOrStore" #key #value
-      {{{ (a: w64) (b: bool), RET (#a, #b); True }}}.
-  Proof. Admitted.
+    {
+      split_and!; auto.
+      - rewrite sh_snoc. unfold sh. word.
+      - apply (next_nibble_extend path h next); try done.
+        + unfold h.
+          pose proof (word.unsigned_range (hash_key key)) as [H0 _].
+          exact H0.
+        + unfold next.
+          rewrite Z2Nat.id; [|word].
+          rewrite <- Z2Nat.id with (n:=sint.Z next_nibble) by word.
+          word.
+      - unfold sh.
+        replace (w64_word_instance.(word.sub) (W64 (64 - 4 * length path)) (W64 4)) with (W64 (64 - 4 * length path - 4)) by word.
+        have Hlt : (length path < 15)%nat.
+        { rewrite app_length /= in Hnext_path_len; lia. }
+        have Hpos : (0 < (64 - 4 * length path - 4))%Z.
+        { lia. }
+        word.
+    }
+
+    Unshelve.
+    {
+      iEval (unfold childP) in "Hchild".
+      rewrite decide_False; [|done].
+      iDestruct "Hchild" as (is_entry) "[#His_entry Hchild]".
+      wp_auto.
+      wp_if_destruct.
+      {
+        wp_apply wp_Bool__Load.
+        iApply fupd_mask_intro; first apply empty_subseteq.
+        iIntros "Hmask".
+        iFrame "Hdead".
+        iIntros "Hdead".
+        iMod "Hmask" as "_".
+        iModIntro.
+        wp_auto.
+        wp_if_destruct.
+        {
+          wp_apply (wp_Mutex__Unlock with "[$Hind_mutex $Hown_mutex $Hdead Hchildren_close Hchild Hown_child]").
+          {
+            iNext.
+            iFrame.
+            rewrite /named.
+            iDestruct ("Hchildren_close" with "[Hchild Hown_child]") as "Hchildren".
+            {
+              iFrame.
+              unfold childP.
+              rewrite decide_False; [|done].
+              iFrame "#".
+              iFrame.
+            }
+            unfold childrenP.
+            iFrame.
+          }
+          wp_for_post.
+          iFrame.
+        }
+        wp_for_post.
+        wp_if_destruct.
+        {
+          wp_apply wp_newEntryNode.
+          iIntros (e n3) "Horphaned_ent".
+          wp_auto.
+          unfold orphaned_entry.
+          iNamed "Horphaned_ent".
+          wp_auto.
+
+          wp_apply wp_Value__Store.
+
+          iInv "Hind_inv" as "HI" "Hclose_ind".
+          iApply fupd_mask_intro; first apply empty_subseteq.
+          iIntros "Hmask".
+          iNext.
+
+          iEval (unfold childrenP) in "HI".
+          iNamedSuffix "HI" "2".
+
+          iDestruct (big_sepL_lookup_acc with "Hchildren2") as "[Hchild2 Hchildren_close2]".
+          { exact Hv. }
+          iNamedSuffix "Hchild2" "2".
+          replace (W64 (sint.nat next_nibble)) with next_nibble by word.
+
+          iDestruct (own_Value_agree with "Hown_child Hown_child2") as %Hneq.
+          inversion Hneq.
+          apply (inj to_val) in H0.
+          subst nodeptr.
+
+          iCombine "Hown_child Hown_child2" as "Hown_child".
+
+          iFrame "Hown_child".
+
+          iIntros "Hown_child".
+
+          iDestruct "Hown_child" as "[Hown_child Hown_child2]".
+
+          (* iMod (inv_alloc entryN _ (entry_inv γ (1/2) (entry γ (1/2)) e path) with "[Hoverflow Hown_path]") as "Hinv". *)
+          (* { *)
+          (*   iNext. *)
+          (*   unfold entry_inv. *)
+          (*   rewrite decide_False; [|exact Hen]. *)
+          (*   (* unfold entry_step. *) *)
+          (*   iExists null. *)
+          (*   rewrite /named. *)
+          (*   iFrame. *)
+          (*   iFrame "#". *)
+          (*   simpl. *)
+          (*   iPureIntro; done. *)
+          (* } *)
+
+          iDestruct (field_pointsto_not_null with "HisEntry") as %Hnn; [simpl; done|auto|].
+
+          iMod (inv_alloc entryN _ (entry_inv γ (1/2) (entry γ (1/2)) e path) with "[]") as "#Hent_inv2".
+          {
+            iNext.
+            unfold entry_inv.
+            rewrite decide_False; [|done].
+            iFrame "#".
+            admit.
+          }
+
+          iDestruct ("Hchildren_close2" with "[Hchild2 Hown_child2]") as "Hchildren2".
+          {
+            iFrame.
+            rewrite /named.
+            unfold childP.
+            iSimpl in "Hchild2".
+            rewrite decide_False; [|exact Hnn].
+            iFrame "#".
+            iExists e.
+            iFrame "#".
+            iSplit; [done|].
+            rewrite entry_unfold /entry_F /named.
+            iFrame "Hent_inv2".
+          }
+
+          admit.
+        }
+        admit.
+      }
+      admit.
+    }
+
+  Admitted.
 
   Lemma wp_HashTrieMap__expand (ht: loc) (oldEntry: loc) (newEntry: loc) (newHash: w64) (hashShift: w64) (parent: loc) :
     {{{ is_pkg_init hashtriemap }}}
@@ -1166,12 +1135,6 @@ Section proof.
     {{{ is_pkg_init hashtriemap }}}
       i @ (ptrT.id hashtriemap.indirect.id) @ "empty" #()
       {{{ (a: bool), RET (#a); True }}}.
-  Proof. Admitted.
-
-  Lemma wp_newEntryNode (key: w64) (value: w64) :
-    {{{ is_pkg_init hashtriemap }}}
-      @! hashtriemap.newEntryNode #key #value
-      {{{ (a: loc), RET (#a); True }}}.
   Proof. Admitted.
 
   Lemma wp_entry__lookupWithValue (e: loc) (key: w64) (value: w64) (checkValue: bool) :
