src/proof/hashtriemap/aux.v
@@ -1,5 +1,7 @@
 (* Things that should be in perennial but arent supported yet *)
 
+From iris.bi.lib Require Import fractional.
+
 From New.generatedproof.hashtriemap Require Import hashtriemap.
 From New.proof Require Import sync.
 From New.proof.sync Require Import atomic.
@@ -14,6 +16,7 @@ From iris.algebra Require Import gmap.
 From iris.base_logic.lib Require Import invariants.
 From stdpp Require Import gmap list fin_maps.
 From Coq Require Import List.
+(* From Perennial.goose_lang Require Import struct. *)
 Import ListNotations.
 Open Scope Z_scope.
 
@@ -28,13 +31,25 @@ Section aux.
   (* go std library potential problem: atomic value doesnt have a nocopy embedded in it because it is older than the atomic integer types (that have the nocopy embedded) *)
   Definition own_Value (u : loc) dq (v : interface.t) : iProp Σ :=
     u ↦{dq} atomic.Value.mk v.
+End aux.
 
-  Notation "l ↦ᵥ{ dq } v" := (own_Value l dq v)
-    (at level 20, format "l  ↦ᵥ{ dq }  v").
+Notation "l ↦ᵥ{ dq } v" := (own_Value l (DfracOwn dq) v)
+                             (at level 20, format "l  ↦ᵥ{ dq }  v").
 
-  Lemma Value_unfold l dq (v : interface.t) :
-    own_Value l dq v ⊣⊢
-    l ↦s[atomic.Value :: "v"]{dq} v.
+Notation "l ↦ᵥ v" := (own_Value l (DfracOwn 1) v)
+                             (at level 20, format "l  ↦ᵥ  v").
+
+Section aux.
+  Context `{hG: heapGS Σ, !invGS Σ, !ffi_semantics _ _}
+    `{!globalsGS Σ} {go_ctx: GoContext}.
+
+  Implicit Types l : loc.
+  Implicit Types u : loc.
+  Implicit Types v : interface.t.
+
+  Lemma Value_unfold l dq v :
+    l ↦ᵥ{dq} v ⊣⊢
+    l ↦s[atomic.Value :: "v"]{DfracOwn dq} v.
   Proof.
     iSplit.
     - iIntros "H".
@@ -45,11 +60,26 @@ Section aux.
       iFrame "Hv".
   Qed.
 
+  Lemma own_Value_agree l dq1 dq2 v1 v2 :
+    l ↦ᵥ{dq1} v1 -∗
+    l ↦ᵥ{dq2} v2 -∗
+    ⌜v1 = v2⌝.
+  Proof.
+    iIntros "H1 H2".
+    iCombine "H1 H2" gives %[? ?].
+    inversion H0.
+    done.
+  Qed.
+
+  Global Instance own_Uint64_fractional u v : Fractional (λ q, u ↦ᵥ{q} v) := _.
+  Global Instance own_Uint64_as_fractional u q v :
+    AsFractional (u ↦ᵥ{q} v) (λ q, u↦ᵥ{q} v) q := _.
+
   (* Using in place of perennial's, since perennial doesnt have std library proofs for atomic Values yet *)
   Lemma wp_Value__Store u v :
     ∀ Φ,
     is_pkg_init atomic -∗
-    (|={⊤,∅}=> ▷ ∃ old, own_Value u (DfracOwn 1) old ∗ (own_Value u (DfracOwn 1) v ={∅,⊤}=∗ Φ #())) -∗
+    (|={⊤,∅}=> ▷ ∃ old, u ↦ᵥ{1} old ∗ (u ↦ᵥ{1} v ={∅,⊤}=∗ Φ #())) -∗
     WP u @ (ptrT.id atomic.Value.id) @ "Store" #v {{ Φ }}.
   Proof.
   Admitted.
@@ -57,18 +87,15 @@ Section aux.
   Lemma wp_Value__Load u dq :
     ∀ Φ,
     is_pkg_init atomic -∗
-    (|={⊤,∅}=> ▷ ∃ v, own_Value u dq v ∗ (own_Value u dq v ={∅,⊤}=∗ Φ #v)) -∗
+    (|={⊤,∅}=> ▷ ∃ v, u ↦ᵥ{dq} v ∗ (u ↦ᵥ{dq} v ={∅,⊤}=∗ Φ #v)) -∗
     WP u @ (ptrT.id atomic.Value.id) @ "Load" #() {{ Φ }}.
   Proof.
   Admitted.
 
-  (* #[global] Instance LoadUint32_Atomic (l:loc) : Atomic StronglyAtomic (atomic.LoadUint32 #l). *)
-  (* Proof. apply _. Qed. *)
-
   (* theres probably already something for this but i couldnt find it *)
   Lemma own_slice_len_keep `{!IntoVal V} `{!IntoValTyped V t} (s: slice.t) dq (vs: list V) :
     s ↦*{dq} vs -∗ s ↦*{dq} vs ∗
-                         ⌜length vs = sint.nat s.(slice.len_f) ∧ 0 ≤ sint.Z s.(slice.len_f)⌝.
+    ⌜length vs = sint.nat s.(slice.len_f) ∧ 0 ≤ sint.Z s.(slice.len_f)⌝.
   Proof.
     iIntros "Hs".
     rewrite own_slice_unseal.
@@ -77,5 +104,5 @@ Section aux.
     iPureIntro.
     split; word.
   Qed.
-  
+
 End aux.
