src/proof/hashtriemap/hashtriemap_done.v
@@ -1,0 +1,1188 @@
+From iris.bi.lib Require Import atomic.
+
+From New.code.hashtriemap Require Import hashtriemap.
+From New.generatedproof.hashtriemap Require Import hashtriemap.
+
+From New.proof Require Import atomic mutex.
+
+From Perennial.algebra Require Import auth_map.
+From Perennial.base_logic.lib Require Import invariants.
+From Perennial.Helpers Require Import NamedProps.
+Import named_props_ascii_notation.
+From Perennial.algebra Require Import ghost_var.
+
+From New.proof.hashtriemap Require Import aux.
+From New.proof.hashtriemap Require Import paths.
+From New.proof.hashtriemap Require Import model.
+
+Open Scope Z_scope.
+
+Section proof.
+  Context `{hG: heapGS Σ, !ffi_semantics _ _}
+    `{!ghost_varG Σ bool}
+    `{!ghost_varG Σ (gmap w64 w64)}
+    `{!mapG Σ w64 w64}
+    `{!mapG Σ Z (gmap w64 w64)}
+    `{!globalsGS Σ} {go_ctx: GoContext}.
+
+  Definition map_get `{!IntoVal V} `{!IntoValTyped V t} (v: option V) : V * bool :=
+    (default (default_val V) v, bool_decide (is_Some v)).
+
+  #[global] Instance : IsPkgInit hashtriemap := define_is_pkg_init True%I.
+  #[global] Instance : GetIsPkgInitWf hashtriemap := build_get_is_pkg_init_wf.
+
+  Lemma next_nibble_eq (key: w64) (path: path) :
+    let h := uint.Z (hash_key key) in
+    let n := w64_word_instance.(word.and)
+                                 (w64_word_instance.(word.sru) (hash_key key)
+                                                      (w64_word_instance.(word.sub) (W64 (sh path)) (W64 4)))
+                                 (W64 15) in
+    length path < 16 → uint.Z n = Z.land (h ≫ (sh path - 4)) 15.
+  Proof.
+    intros.
+    (* subst n. *)
+    (* zify. *)
+    unfold h.
+    rewrite word.unsigned_and_nowrap.
+    rewrite word.unsigned_sru.
+    - rewrite word.unsigned_sub.
+      f_equiv; [|word].
+      unfold sh.
+      rewrite wrap_small; auto.
+      + f_equiv.
+        word.
+      + replace (uint.Z (W64 (64 - 4 * length path))) with (64 - 4 * length path) by word.
+        replace (uint.Z (W64 4)) with 4 by word.
+        replace (w64_word_instance_ok.(word.wrap) (64 - 4 * length path - 4)) with (64 - 4 * length path - 4) by word.
+        unfold sh in *.
+        have Hx : ((64 - 4 * length path - 4)) ≥ 0 by lia.
+        have Hrng : 0 ≤ uint.Z (hash_key key) < 2^64 by word.
+        split.
+        * apply Z.shiftr_nonneg. lia.
+        * destruct Hrng as [_ Hrng].
+          apply (Z.le_lt_trans _ (uint.Z (hash_key key))); [|exact Hrng].
+          set x := uint.Z (hash_key key).
+          rewrite Z.shiftr_div_pow2; [|word].
+          apply Z.div_le_upper_bound; [word|].
+          set z := 2 ^ (64 - 4 * length path - 4).
+          have Hz : 1 ≤ z.
+          {
+            replace 1 with (2^0) by lia.
+            apply Z.pow_le_mono_r; lia.
+          }
+          replace (z * x) with (x * z) by lia.
+          clear Hx.
+          have Hx : 0 ≤ x by word.
+          have Hy : 1 ≤ z by lia.
+          have : x * 1 ≤ x * z.
+          { apply (Z.mul_le_mono_nonneg_l _ _ _ Hx).
+            exact Hy. }
+          word.
+    - replace (w64_word_instance.(word.sub) (W64 (sh path)) (W64 4)) with (W64 (sh path - 4)) by word.
+      unfold sh.
+      replace (uint.Z (W64 (64 - 4 * length path - 4))) with (64 - 4 * length path - 4) by word.
+      word.
+  Qed.
+
+  Lemma wp_node__entry (n: loc) (e: loc) :
+    {{{ is_pkg_init hashtriemap ∗
+        n ↦s[hashtriemap.node :: "isEntry"]□ true ∗
+        n ↦s[hashtriemap.node :: "ent"]□ e }}}
+      n @ (ptrT.id hashtriemap.node.id) @ "entry" #()
+      {{{ RET #e; True }}}.
+  Proof.
+    wp_start as "(His_entry & Hent)".
+    wp_auto.
+    iApply "HΦ"; done.
+  Qed.
+
+  Lemma wp_node__indirect (n: loc) (i: loc) :
+    {{{ is_pkg_init hashtriemap ∗
+        n ↦s[hashtriemap.node :: "isEntry"]□ false ∗
+        n ↦s[hashtriemap.node :: "ind"]□ i }}}
+      n @ (ptrT.id hashtriemap.node.id) @ "indirect" #()
+      {{{ RET #i; True }}}.
+  Proof.
+    wp_start as "(His_entry & Hind)".
+    wp_auto.
+    iApply "HΦ"; done.
+  Qed.
+
+  (* precondition: returns value, true if k is in kvs *)
+  Lemma wp_entry__lookup (ht: loc) (e: loc) (key: K) (γ: ghost_names) (path: path) :
+    ∀ (Φ: val → iProp Σ),
+    is_pkg_init hashtriemap -∗
+    "Hpre" :: (
+        "#His_map" :: is_hashtriemap γ ht ∗
+        "%Hen" ∷ ⌜e ≠ null⌝ ∗
+        "Hentry" :: entry γ (1 / 2) e path ∗
+        "Hau" :: (AU <{ ∃∃ m, own_ht_map γ m }>
+                    @ ht_au_mask, ∅
+                  <{ own_ht_map γ m, COMM Φ (ht_load_ret m key) }>) ∗
+        "%Hbelongs" :: ⌜belongs_to_path path (uint.Z (hash_key key))⌝
+      ) -∗
+    WP e @ (ptrT.id hashtriemap.entry.id) @ "lookup" #key {{ Φ }}.
+  Proof.
+    intros.
+    set h := (uint.Z (hash_key key)).
+    iIntros.
+    iNamed.
+    iNamed "Hpre".
+    wp_method_call. wp_call.
+
+    wp_auto.
+
+    iAssert (
+        ∃ e,
+          "e" :: e_ptr ↦ e ∗
+          "Hentry" ::
+            if decide (e = null) then
+              Φ (ht_load_ret ∅ key)
+            else
+              "Hau" ∷ (AU <{ ∃∃ m, own_ht_map γ m }>
+                         @ ht_au_mask, ∅
+                                       <{ own_ht_map γ m, COMM Φ (ht_load_ret m key) }>) ∗
+              "Hentry" ∷ entry γ (1 / 2) e path
+      )%I with "[$e Hentry Hau]" as "Hloop".
+    { rewrite decide_False; [iFrame|done]. }
+    clear Hen e.
+
+    wp_for "Hloop".
+
+    wp_if_destruct.
+    {
+      wp_alloc ret as "ret".
+      wp_auto.
+      unfold ht_load_ret.
+      iSimpl in "Hentry".
+      iApply "Hentry".
+    }
+
+    iRevert "Hentry".
+    rewrite decide_False; [|exact n].
+    iIntros "Hentry".
+    iNamed "Hentry".
+
+    (* { *)
+    (*   iApply wp_fupd. *)
+    (*   wp_alloc ret as "ret". *)
+    (*   wp_auto. *)
+
+    (*   (* iEval (rewrite decide_False) in "Hentry". *) *)
+    (*   iEval (rewrite entry_unfold /entry_F) in "Hentry". *)
+    (*   iNamed "His_map". *)
+    (*   iInv "His_map" as (rooti hm user_map) "(>? & >? & >? & #Hroot_indirect & >? & >? & >?)" "Hclose_map". *)
+    (*   iNamed. *)
+    (*   iInv "Hentry_inv" as "HEI" "Hclose_entry". *)
+    (*   unfold entry_inv. *)
+    (*   iSimpl in "HEI". *)
+    (*   iMod "HEI" as "Hown_empty". *)
+    (* (* iDestruct "HEI" as (next k v h0 rest_map) "(>? & >? & >? & >? & >? & >? & HEI)". *) *)
+    (* (* iNamed. *) *)
+    (*   (* iInv "Hentry_inv" as "HEI" "Hclose_entry". *) *)
+    (*   (* unfold entry_inv. *) *)
+    (*   (* iEval (simpl) in "HEI". *) *)
+    (*   (* iMod "HEI". *) *)
+    (*   (* iNamed. *) *)
+    (*   (* iMod (fupd_mask_subseteq (⊤ ∖ ↑mapN ∖ ↑indN ∖ ↑entryN)) as "Hclose_au_mask"; [set_solver|]. *) *)
+    (*   iMod "Hau" as (m) "[Hown Hclose_au]". *)
+
+    (*   iDestruct (ghost_var_agree with "Hown Huser_map") as %Heq. *)
+    (*   subst m. *)
+
+    (*   have Hdom : h ∈ path_to_domain path. *)
+    (*   { *)
+    (*     rewrite list_elem_of_filter. *)
+    (*     split; [exact Hbelongs|]. *)
+    (*     apply full_domain_elem. *)
+    (*   } *)
+
+    (*   iDestruct (own_path_lookup _ _ _ h with "Hown_empty") as "[Hptsto Hptsto_close]"; [exact Hdom|]. *)
+    (*   iDestruct (map_valid with "Hauth_map Hptsto") as %Hlookup. *)
+    (*   iDestruct ("Hptsto_close" with "Hptsto") as "Hown_empty". *)
+
+    (*   have Hnone : user_map !! key = None. *)
+    (*   { *)
+    (*     rewrite Hflat. *)
+    (*     rewrite (Hbuckets _ _ _ Hlookup); done. *)
+    (*   } *)
+
+    (*   iNamed. *)
+
+    (*   iMod ("Hclose_au" with "[$]") as "HΦ". *)
+    (*   (* iMod "Hclose_au_mask" as "_". *) *)
+    (*   iMod ("Hclose_entry" with "[Hown_empty]") as "_"; [iNext; done|]. *)
+    (*   iMod ("Hclose_map" with "[$Hauth_map $Hown_root $Hroot_indirect $Hown //]") as "_". *)
+    (*   iApply fupd_mask_intro; [set_solver|]. *)
+    (*   iIntros "_". *)
+    (*   unfold ht_load_ret. *)
+    (*   iEval (rewrite Hnone; simpl) in "HΦ". *)
+    (*   iApply "HΦ". *)
+    (* } *)
+
+    iApply fupd_wp.
+    rewrite entry_unfold /entry_F.
+    iNamed.
+
+    iInv "Hentry_inv" as "HEI" "Hclose_entry".
+    unfold entry_inv.
+    destruct (decide (e = null)); [exfalso; auto|].
+    iDestruct "HEI" as (next k v h0 rest_map) "(>? & >? & >? & >? & >? & >? & HEI)".
+    iNamed.
+
+    destruct (bool_decide (k = key)) eqn:Heq_key.
+    - apply bool_decide_eq_true in Heq_key.
+      replace h0 with h by (unfold h; subst; reflexivity).
+
+      iNamed "His_map".
+      iInv "His_map" as (rooti hm user_map) "(>? & >? & >? & #Hroot_indirect & >? & >? & >?)" "Hclose_map".
+      iNamed.
+      iMod (fupd_mask_subseteq (⊤ ∖ ↑mapN ∖ ↑indN ∖ ↑entryN)) as "Hclose_au_mask"; [set_solver|].
+      iMod "Hau" as (m) "[Hown Hclose_au]".
+
+      (* linearization point *)
+
+      iDestruct (ghost_var_agree with "Hown Huser_map") as %Heq.
+      subst m.
+
+      have Hdom : h ∈ path_to_domain path.
+      {
+        rewrite list_elem_of_filter.
+        split; [exact Hbelongs|].
+        apply full_domain_elem.
+      }
+
+      iDestruct (own_path_lookup _ _ _ h with "Hown_path") as "[Hptsto Hptsto_close]"; [exact Hdom|].
+      iDestruct (map_valid with "Hauth_map Hptsto") as %Hlookup.
+      iDestruct ("Hptsto_close" with "Hptsto") as "Hown_path".
+
+      have Hsome : user_map !! key = Some v.
+      {
+        subst k.
+        rewrite Hflat.
+        rewrite (Hbuckets _ _ _ Hlookup); try done.
+        unfold singleton_map_fn.
+        rewrite decide_True; [|done].
+        rewrite lookup_insert.
+        rewrite decide_True; done.
+      }
+
+      iNamed.
+
+      iMod ("Hclose_au" with "[$]") as "HΦ".
+
+      iMod "Hclose_au_mask" as "_".
+      iMod ("Hclose_map" with "[$Hauth_map $Hown_root $Hroot_indirect $Hown //]") as "_".
+      iMod ("Hclose_entry" with "[$Hown_path $HEI $Hown_next]") as "_".
+      {
+        iNext.
+        iFrame "#".
+        iPureIntro; subst k; done.
+      }
+
+      iApply fupd_mask_intro; [set_solver|].
+      iIntros "_".
+      wp_auto.
+      wp_if_destruct; [|exfalso; auto].
+
+      wp_for_post.
+
+      unfold ht_load_ret.
+
+      iEval (rewrite Hsome; simpl) in "HΦ".
+      iApply "HΦ".
+    - apply bool_decide_eq_false in Heq_key.
+
+      iMod ("Hclose_entry" with "[$Hown_path $HEI $Hown_next]") as "_";
+        [ iNext; iFrame "#"; iPureIntro; done |].
+
+      iApply fupd_mask_intro; [set_solver|].
+      iIntros "_".
+
+      wp_auto.
+
+      wp_if_destruct; [exfalso; auto|].
+      clear n1.
+      wp_apply wp_Value__Load.
+
+      iInv "Hentry_inv" as "HEI" "Hclose_entry".
+      unfold entry_inv.
+      destruct (decide (e = null)); [exfalso; auto|].
+      iDestruct "HEI" as "HEI".
+      iNamed "HEI".
+      iDestruct "HEI" as (next0 k0 v0 h0 rest_map0) "(>Hk0 & >Hv0 & >? & >? & >? & >? & HEI)".
+
+      iNamedSuffix "Hk0" "0".
+      iCombine "Hk" "Hk0" gives %[? ?].
+
+      iClear "Hk".
+      iClear "Hv".
+      subst k.
+      (* clear Hbelongs. *)
+      (* rename Hbelongs0 into Hbelongs. *)
+      (* clear Heq_key. *)
+      clear n0.
+      clear next.
+      rename next0 into next.
+      clear v rest_map.
+      iNamed.
+
+      destruct (decide (e = null)); [exfalso; auto|].
+
+      iApply fupd_mask_intro; [set_solver|].
+      iIntros "Hmask".
+      iNext.
+
+      (* iNamedSuffix "Hk0" "0". *)
+      (* iNamedSuffix "Hv0" "0". *)
+      iNamed.
+      iFrame "Hown_next".
+      iIntros "Hown_next".
+
+      destruct (decide (next = null)) eqn:Heq_next.
+      + iNamed "His_map".
+        iMod "Hmask" as "_".
+        iInv "His_map" as (rooti hm user_map) "(>? & >? & >? & #Hroot_indirect & >? & >? & >?)" "Hclose_map".
+        iNamed.
+        iMod "Hau" as (m) "[Hown Hclose_au]".
+
+        iDestruct (ghost_var_agree with "Hown Huser_map") as %Heq.
+        subst m.
+
+        have Hdom : h ∈ path_to_domain path.
+        {
+          rewrite list_elem_of_filter.
+          split; [exact Hbelongs|].
+          apply full_domain_elem.
+        }
+
+        iDestruct "HEI" as %Hrest_null.
+        subst rest_map0.
+
+        iDestruct (own_path_lookup _ _ _ h with "Hown_path") as "[Hptsto Hptsto_close]"; [exact Hdom|].
+        iDestruct (map_valid with "Hauth_map Hptsto") as %Hlookup.
+        iDestruct ("Hptsto_close" with "Hptsto") as "Hown_empty".
+
+        have Hnone : user_map !! key = None.
+        {
+          rewrite Hflat.
+          rewrite (Hbuckets _ _ _ Hlookup); [|done].
+          unfold singleton_map_fn.
+          destruct (decide (h = h0)).
+          - rewrite lookup_insert.
+            rewrite decide_False; done.
+          - rewrite lookup_empty.
+            done.
+        }
+
+        iNamed.
+
+        iMod ("Hclose_au" with "[$]") as "HΦ".
+        iMod ("Hclose_map" with "[$Hauth_map $Hown_root $Hroot_indirect $Hown //]") as "_".
+        iMod ("Hclose_entry" with "[Hown_empty Hown_next]") as "_".
+        {
+          iNext.
+          iFrame.
+          iFrame "#".
+          rewrite decide_True; done.
+        }
+        iApply fupd_mask_intro; [set_solver|].
+        iIntros "_".
+        unfold ht_load_ret.
+        iEval (rewrite Hnone; simpl) in "HΦ".
+        wp_apply wp_interface_type_assert; [auto|].
+
+        wp_for_post.
+        iFrame.
+        rewrite decide_True; [|exact e0].
+        iFrame "HΦ".
+      + iNamed "HEI".
+
+        iMod "Hmask" as "_".
+        iMod ("Hclose_entry" with "[$Hown_path $Hown_next]") as "_".
+        {
+          iNext.
+          rewrite decide_False; [|exact n2].
+          iFrame "#".
+          iPureIntro; done.
+        }
+
+        iApply fupd_mask_intro; [set_solver|].
+        iIntros "_".
+
+        wp_apply wp_interface_type_assert; [auto|].
+
+        wp_for_post.
+        iFrame.
+        rewrite decide_False; [|exact n2].
+        iFrame "Hau".
+        iFrame "Hnext_entry".
+  Qed.
+
+  Lemma wp_hashInt (key: w64) (seed: w64) :
+    {{{ is_pkg_init hashtriemap }}}
+      @! hashtriemap.hashInt #key #seed
+      {{{ (a: w64), RET (#a); ⌜a = hash_key key⌝ }}}.
+  Proof. Admitted.
+
+  Lemma wp_newIndirectNode (γ: ghost_names) (parent: loc) (path: list Z) (hm: hash_map) :
+    {{{ is_pkg_init hashtriemap }}}
+      @! hashtriemap.newIndirectNode #parent
+      {{{ (ind: loc), RET (#ind);
+          indirect γ ind path }}}.
+  Proof.
+    wp_start as "Hpre".
+    wp_auto.
+    rename i_ptr into ind_ptr.
+    iRename "i" into "ind".
+
+    wp_apply (wp_slice_make2 (V:=atomic.Value.t)).
+    { unfold hashtriemap.nChildren. word. }
+    iIntros (children) "(Hchildren & _)".
+    wp_auto.
+    wp_alloc ind_struct as "ind_struct".
+    wp_auto.
+
+    set (children_vs := replicate (sint.nat (W64 hashtriemap.nChildren))
+                          atomic.into_val_typed_Value.(default_val atomic.Value.t)).
+
+    iAssert (
+        ∃ (vs: list atomic.Value.t) (idx i: w64),
+          "Hvs" :: children ↦* vs ∗
+          "i" :: i_ptr ↦ i ∗
+          "idx" :: idx_ptr ↦ idx ∗
+          "%Hi_idx" :: ⌜sint.Z i >= sint.Z idx⌝ ∗
+          "%Hi_bound" :: ⌜uint.Z i <= hashtriemap.nChildren⌝ ∗
+          "%Hlen" :: ⌜length vs = Z.to_nat hashtriemap.nChildren⌝ ∗
+          "%Hprefix" :: ⌜∀ (j: nat), j ≥ 0 → j < uint.Z i →
+                                     ∃ av, vs !! j = Some av ∧
+                                           av = atomic.Value.mk (interface.mk (ptrT.id hashtriemap.node.id) (# null))⌝ ∗
+                                           "%Hsuffix" :: ⌜∀ (j: nat), j >= uint.Z i → j < length vs → vs !! j = children_vs !! j⌝
+      )%I with "[$Hchildren $i $idx]" as "IH".
+    {
+      iNamed.
+      unfold hashtriemap.nChildren.
+      iPureIntro.
+      simpl.
+      split_and!; auto; try word.
+      iIntros (j Hj Hj2).
+      exfalso.
+      word.
+    }
+
+    wp_for "IH".
+
+    iDestruct (own_slice_len_keep with "Hvs") as "(Hvs & %Hlen_slice & _)".
+
+    wp_if_destruct.
+    2: {
+      wp_alloc node as "node".
+
+      iApply struct_fields_split in "ind_struct".
+      iNamed "ind_struct".
+      iApply struct_fields_split in "node".
+      iNamed "node".
+      simpl.
+      wp_auto.
+
+      iAssert (
+          indirect γ ind_struct path
+        )%I with "[Hvs Hnode Hdead Hmu Hparent Hchildren HisEntry Hent Hind]" as "Hinv".
+      {
+        (* TODO: whatever this invariant ends up being, need to prove it here with M=∅ *)
+        admit.
+      }
+
+      iApply "HΦ".
+      iFrame "Hinv".
+    }
+
+    wp_pure.
+    { split; word. }
+
+    have Hlookup_vs : (vs !! sint.nat i = Some (atomic.into_val_typed_Value.(default_val atomic.Value.t))).
+    {
+      have Hidx_lt : uint.nat i < length vs.
+      { rewrite Hlen. word. }
+
+      have Hsuffix_i : vs !! uint.nat i = children_vs !! uint.nat i.
+      { apply Hsuffix; [lia|exact Hidx_lt]. }
+
+      have Hsuit : sint.nat i = uint.nat i.
+      { word. }
+
+      rewrite Hsuit.
+      rewrite Hsuffix_i.
+      rewrite lookup_replicate_2; auto.
+      word.
+    }
+
+    wp_apply (wp_load_slice_elem with "[$Hvs]"); auto.
+    { word. }
+
+    iIntros "Hvs".
+
+    wp_auto.
+
+    wp_pure.
+    { split; cbn; word. }
+
+    wp_auto.
+
+    iDestruct ((own_slice_elem_acc) with "[$Hvs]") as "[Helem Hcont]"; eauto.
+    { word. }
+
+    iAssert (own_Value (slice.elem_ref_f children atomic.Value i) 1 interface.nil)%I
+      with "[Helem]" as "Helem".
+    {
+      auto.
+    }
+
+    wp_apply wp_Value__Store.
+
+    iApply fupd_mask_intro.
+    { set_solver. }
+    iIntros "Hmask".
+    iNext.
+    iFrame "Helem".
+    iIntros "Helem".
+    iMod "Hmask".
+    iClear "Hmask".
+    iApply fupd_mask_intro.
+    {set_solver. }
+    iIntros "_".
+    wp_auto.
+
+    iDestruct ("Hcont" with "Helem") as "Hvs".
+
+    wp_for_post.
+
+    iFrame "HΦ ind ind_struct".
+
+    iFrame.
+
+    iSplit.
+    { word. }
+
+    iSplit.
+    { word. }
+    iSplit.
+    {
+      iPureIntro.
+      rewrite length_insert.
+      exact Hlen.
+    }
+    iSplit.
+    - iPureIntro. intros j Hj_ge Hj_lt.
+
+      have Hj_lte : j ≤ uint.Z i.
+      { word. }
+      clear Hj_lt.
+
+      apply Z_le_lt_eq_dec in Hj_lte.
+      destruct Hj_lte as [Hlt | Heq].
+
+      + (* j < i *)
+        specialize (Hprefix j) as Hprefix.
+        specialize (Hprefix Hj_ge Hlt).
+        destruct Hprefix as (av & Hlookup & Hav).
+        exists av.
+        split; auto.
+
+        rewrite list_lookup_insert_ne; auto.
+        word.
+      + (* j = i *)
+        exists {| atomic.Value.v' := interface.mk (ptrT.id hashtriemap.node.id) (# null) |}.
+        split; auto.
+        rewrite list_lookup_insert.
+        have Hbool : (sint.nat i = j ∧ (sint.nat i < length vs)%nat)%nat.
+        { word. }
+        by destruct (decide (sint.nat i = j ∧ (sint.nat i < length vs)%nat)) as [H|H];
+        [reflexivity | exfalso; exact (H Hbool)].
+    - iPureIntro. intros j Hj_ge Hj_lt.
+
+      have Hj_ge_i1_nat : (j ≥ uint.nat i + 1)%nat.
+      { word. }
+      have Hj_ge_i_Z : (j >= uint.Z i).
+      { word. }
+      have Hj_ge_i1_Z : (j >= uint.Z i + 1).
+      { word. }
+      have Hj_lt_len : (j < length vs).
+      { rewrite length_insert in Hj_lt. word. }
+
+      specialize (Hsuffix j) as Hsuffix.
+      specialize (Hsuffix Hj_ge_i_Z Hj_lt_len).
+      rewrite list_lookup_insert_ne; auto.
+      word.
+  Admitted.            (* only admitted because of the ind invariant needing proof *)
+
+  Lemma wp_HashTrieMap__initSlow (ht: loc) (γ: ghost_names) :
+    {{{ is_pkg_init hashtriemap ∗ is_pkg_init atomic ∗ is_pkg_init sync ∗
+        hashtriemap_init ht γ }}}
+      ht @ (ptrT.id hashtriemap.HashTrieMap.id) @ "initSlow" #()
+      {{{ RET #();
+          "His_map" :: is_hashtriemap γ ht }}}.
+  Proof.
+    wp_start as "Hpre".
+    iNamed "Hpre".
+    iRename "Hinit_mu" into "Hmu".
+
+    wp_apply wp_with_defer as "%defer defer"; simpl subst.
+    wp_auto.
+
+    wp_apply (wp_Mutex__Lock with "[$Hmu]").
+    iIntros "(Hown_mutex&Hmu_inv)".
+    wp_auto.
+
+    wp_apply wp_Uint32__Load.
+    iInv "Hinit" as (b) "(>Hinited & >Hinit_tok & #Hstatus_done)" "Hclose".
+    iApply fupd_mask_intro.
+    { set_solver. }
+    iIntros "Hmask".
+    iNext.
+    iFrame.
+
+    iIntros "Hinited".
+
+    iDestruct (persistently_elim with "Hstatus_done") as "#Hstatus_done'".
+    iClear "Hstatus_done".
+    iRename "Hstatus_done'" into "Hstatus_done".
+
+    destruct b; simpl in *.
+    {
+      iMod "Hmask".
+      iClear "Hmask".
+      iMod ("Hclose" with "[Hinit_tok Hinited Hstatus_done]") as "_".
+      { iNext; iFrame; iFrame "Hinited Hstatus_done". }
+      iApply fupd_mask_intro.
+      { set_solver. }
+      iIntros "_".
+      wp_auto.
+
+      wp_apply (wp_Mutex__Unlock with "[$Hmu $Hown_mutex $Hmu_inv]").
+
+      iApply "HΦ"; done.
+    }
+
+    iDestruct "Hmu_inv" as (b) "Hmu_inv".
+    destruct b.
+    {
+      iDestruct (ghost_var_agree with "Hmu_inv Hinit_tok") as %Heq.
+      inversion Heq.
+    }
+
+    iMod "Hmask".
+    iClear "Hmask".
+    iMod ("Hclose" with "[Hinit_tok Hinited Hstatus_done]") as "_".
+    { iNext; iFrame; iFrame "Hstatus_done Hinited". }
+    iApply fupd_mask_intro.
+    { set_solver. }
+    iIntros "_".
+    wp_auto.
+
+    (* TODO: have lemma to initialize empty_map, and give the ptsto_mut part to newIndirectNode and the auth_map used for constructing ht_inv below *)
+    wp_apply (wp_newIndirectNode γ null [] ∅).
+    iIntros (root_node_ptr) "root_node".
+    wp_auto.
+
+    iFrame.
+    wp_apply wp_Value__Store.
+
+    iInv "Hinit" as (b) "(>Hinited & >Hinit_tok & _)" "Hclose".
+    iApply fupd_mask_intro; [set_solver|].
+    iIntros "Hmask".
+    iNext.
+    iFrame.
+    iExists interface.nil.
+
+    iDestruct "Hmu_inv" as "(Hinit_tok2 & Hseed & Hroot)".
+    iDestruct (ghost_var_agree with "Hinit_tok Hinit_tok2") as %Heq.
+    subst b.
+
+    iFrame.
+
+    iIntros "Hroot".
+    iMod "Hmask".
+    iClear "Hmask".
+    iMod ("Hclose" with "[Hinit_tok Hinited Hstatus_done]") as "_".
+    {
+      iNext.
+      iFrame.
+      iFrame "Hstatus_done Hinited".
+    }
+
+    iApply fupd_mask_intro.
+    { set_solver. }
+    iIntros "_".
+    wp_auto.
+
+    iDestruct "Hseed" as (seed) "Hseed".
+
+    wp_apply (wp_store_ty with "Hseed").
+    Unshelve.
+    2: { eapply into_val_typed_w64. }
+
+    iIntros "Hseed".
+    iPersist "Hseed".
+
+    wp_auto.
+    wp_apply wp_Uint32__Store.
+
+    iInv "Hinit" as (b) "(>Hinited & >Hinit_tok & _)" "Hclose".
+    iApply fupd_mask_intro.
+    { set_solver. }
+    iIntros "Hmask".
+    iNext.
+    iFrame.
+    iIntros "Hinited".
+    iMod "Hmask".
+    iClear "Hmask".
+    destruct b.
+    {
+      iDestruct (ghost_var_agree with "Hinit_tok Hinit_tok2") as %Heq.
+      exfalso. congruence.
+    }
+
+    iMod (ghost_var_update_halves true with "Hinit_tok Hinit_tok2") as "(Htok1 & Htok2)".
+
+    iAssert (ht_inv ht γ)%I (* with "[$]" *) as "Hhtinv".
+    {
+      admit.
+    }
+
+    iMod (invariants.inv_alloc mapN _ (
+              "Hinv" :: ht_inv ht γ
+            ) with "[$Hhtinv]") as "#His_map".
+
+    iMod ("Hclose" with "[Htok1 Hinited His_map]") as "_".
+    { iNext. iFrame. iFrame "Hinited". unfold init_status_done. iFrame "His_map Hseed". }
+    iApply fupd_mask_intro.
+    {set_solver. }
+    iIntros "_".
+    wp_auto.
+
+    iAssert (init_mu_inv ht γ)%I with "[Htok2]" as "Hmu_inv_true".
+    { simpl. iExists true. iFrame "Htok2". }
+
+    wp_apply (wp_Mutex__Unlock with "[$Hmu $Hown_mutex $Hmu_inv_true]").
+    iApply "HΦ".
+    iFrame.
+    unfold is_hashtriemap.
+    iFrame "#".
+  Admitted.
+
+  (*precondition: either inited is 0 and we call initSlow, or its 1 and we already have the initialization requirements*)
+  Lemma wp_HashTrieMap__initHT (ht: loc) (γ: ghost_names) :
+    {{{ is_pkg_init hashtriemap ∗ is_pkg_init atomic ∗ is_pkg_init sync ∗
+        hashtriemap_init ht γ }}}
+      ht @ (ptrT.id hashtriemap.HashTrieMap.id) @ "initHT" #()
+      {{{ RET #();
+          "His_map" :: is_hashtriemap γ ht }}}.
+  Proof.
+    wp_start as "Hpre".
+    iNamed "Hpre".
+    iRename "Hinit_mu" into "Hmu".
+
+    wp_auto.
+
+    wp_apply wp_Uint32__Load.
+    iInv "Hinit" as "Hinit2" "Hclose".
+    iApply fupd_mask_intro.
+    { set_solver. }
+    iIntros "Hmask".
+    iNext.
+    iDestruct "Hinit2" as (b) "(Hinited & Hinit_tok & #Hstatus_done)".
+    iFrame.
+    iIntros "Hinited".
+    iMod "Hmask".
+    iClear "Hmask".
+    iMod ("Hclose" with "[Hinit_tok Hinited Hstatus_done]") as "_".
+    { iNext. iFrame. iFrame "Hstatus_done". }
+    iApply fupd_mask_intro.
+    { set_solver. }
+    iIntros "_".
+    wp_auto.
+
+    wp_if_destruct.
+    - wp_apply (wp_HashTrieMap__initSlow).
+      { iFrame. iFrame "Hinit Hmu". }
+      iIntros.
+      wp_auto.
+      iApply "HΦ".
+      iFrame "#".
+    - iApply "HΦ".
+      iFrame.
+      destruct b; simpl.
+      + iFrame "#".
+      + exfalso. congruence.
+  Qed.
+
+  (* dont actually need the is_hashtriemap precondition for any of the lemmas because initHT gives it to us *)
+  Lemma wp_HashTrieMap__Load (ht: loc) (key: w64) (γ: ghost_names) :
+    ∀ (Φ: val → iProp Σ),
+    (is_pkg_init hashtriemap ∗ is_pkg_init atomic ∗ is_pkg_init sync ∗
+     "Hinit" :: hashtriemap_init ht γ ∗
+     "Hau" ::
+       AU <{ ∃∃ m : gmap K V, own_ht_map γ m }>
+       @ ht_au_mask, ∅
+                     <{ own_ht_map γ m, COMM Φ (ht_load_ret m key) }>) -∗
+    WP ht @ (ptrT.id hashtriemap.HashTrieMap.id) @ "Load" #key {{ Φ }}.
+  Proof.
+    iIntros (Φ) "(#? & #? & #? & Hpre)".
+    iNamed "Hpre".
+
+    wp_method_call. wp_call.
+
+    wp_auto.
+
+    wp_apply (wp_HashTrieMap__initHT with "[$]").
+    iIntros.
+    iNamed.
+    iNamed "His_map".
+    wp_auto.
+
+    wp_apply wp_hashInt.
+    iIntros (hash) "%Hhash".
+
+    wp_auto.
+
+    wp_apply wp_Value__Load.
+    iInv "His_map" as "Hhtinv" "Hclose".
+    iApply fupd_mask_intro.
+    { set_solver. }
+    iIntros "Hmask".
+    iNext.
+    iNamed "Hhtinv".
+    iEval (unfold ht_inv) in "Hinv".
+    iNamed "Hinv".
+    iFrame "Hown_root".
+    iIntros "Hown_root".
+    iMod "Hmask".
+    iClear "Hmask".
+
+    unfold ht_inv.
+    iMod ("Hclose" with "[$Hauth_map $Huser_map $Hown_root $Hroot_indirect]") as "_"; [iNext; iPureIntro; done|].
+
+    iApply fupd_mask_intro.
+    { set_solver. }
+    iIntros "_".
+
+    clear Hflat.
+    clear Hbuckets Hbuckets_rev.
+    clear hm. clear user_map.
+
+    wp_apply wp_interface_type_assert.
+    { auto. }
+
+    set h := uint.Z (hash_key key).
+
+    iAssert (∃ (path: path) (shift: w64) (cur: loc),
+                "Hcur" :: i_ptr ↦ cur ∗
+                "Hhash_shift" :: hashShift_ptr ↦ shift ∗
+                "#Hi_indirect" :: indirect γ cur path ∗
+                "%Hshift" :: ⌜shift = sh path⌝ ∗
+                "%Hpath_len" :: ⌜length path < 16⌝ ∗
+                "%Hkey_path" :: ⌜belongs_to_path path h⌝
+            )%I with ("[$Hroot_indirect $hashShift $i]") as "Hloop_inv".
+    {
+      repeat iSplit; eauto.
+      iPureIntro.
+      unfold belongs_to_path, sh, path_to_prefix.
+      simpl.
+      rewrite Z.shiftr_div_pow2; try word.
+    }
+    iClear "Hroot_indirect".
+
+    wp_for "Hloop_inv".
+
+    iEval (rewrite indirect_unfold /indirect_F) in "Hi_indirect".
+    iNamed "Hi_indirect".
+
+    wp_if_destruct.
+    {
+      wp_apply wp_panic.
+      iPureIntro.
+      unfold sh in e.
+      word.
+    }
+
+    iDestruct (own_slice_len with "Hchildren_slice") as "(%Hlen_children_16 & _)".
+    have Hlen_children : uint.Z children_slice.(slice.len_f) = 16.
+    { word. }
+    clear Hlen_children_16.
+
+    unfold hashtriemap.nChildrenLog2, hashtriemap.nChildrenMask in *.
+    wp_pure.
+    {
+      have Hlen16 : uint.Z children_slice.(slice.len_f) = 16 by word.
+      set (x := w64_word_instance.(word.sru) (hash_key key)
+                                    (w64_word_instance.(word.sub) (W64 (64 - 4 * length path)) (W64 4))).
+      have Hnib_u : 0 ≤ uint.Z (w64_word_instance.(word.and) x (W64 15)) < 16.
+      {
+        rewrite word.unsigned_and_nowrap.
+        change (uint.Z (W64 15)) with 15.
+        change 15 with (Z.ones 4).
+        rewrite Z.land_ones; word.
+      }
+      have Hsint :
+        sint.Z (w64_word_instance.(word.and) x (W64 15)) =
+        uint.Z (w64_word_instance.(word.and) x (W64 15)).
+      { word. }
+      rewrite Hsint.
+      word.
+    }
+
+    set next_nibble := (w64_word_instance.(word.and)
+                                            (w64_word_instance.(word.sru)
+                                                                 (hash_key key)
+                                                                 (w64_word_instance.(word.sub)
+                                                                                      (W64 (sh path))
+                                                                                      (W64 4)))
+                                            (W64 15)).
+
+    have Hnib_u : 0 ≤ uint.Z next_nibble < 16.
+    {
+      unfold next_nibble.
+      rewrite word.unsigned_and_nowrap.
+      change (uint.Z (W64 15)) with 15.
+      split.
+      - apply Z.land_nonneg.
+        right.
+        word.
+      - change 15 with (Z.ones 4).
+        rewrite Z.land_ones.
+        + apply Z_mod_lt.
+          word.
+        + word.
+    }
+
+    have Hlt_nat : (sint.nat next_nibble < length children_vals)%nat by
+                     (rewrite Hchildren_len; word).
+    destruct (lookup_lt_is_Some_2 children_vals (sint.nat next_nibble) Hlt_nat)
+      as [v Hv].
+
+    wp_auto.
+
+    have Hdom : h ∈ path_to_domain path.
+    {
+      unfold path_to_domain.
+      rewrite list_elem_of_filter.
+      split.
+      - exact Hkey_path.
+      - apply full_domain_elem.
+    }
+
+    wp_apply wp_Value__Load.
+    iInv "His_map" as "Hhtinv" "Hclose_ht".
+    iInv "Hind_inv" as "HI" "Hclose_ind".
+
+    unfold own_ht_map.
+    iApply fupd_mask_intro.
+    { apply empty_subseteq.
+    (* set_solver. doesnt work, only when Hdom is defined? *) }
+    iIntros "Hmask".
+    iNext.
+
+    iEval (unfold childrenP) in "HI".
+
+    iNamed "HI".
+
+    iNamed "Hhtinv".
+    iNamed "Hinv".
+
+    iDestruct (big_sepL_lookup_acc with "Hchildren") as "[Hchild Hchildren_close]".
+    { exact Hv. }
+    iNamed "Hchild".
+    iExists (interface.mk (ptrT.id hashtriemap.node.id) (# nodeptr)).
+    replace (W64 (sint.nat next_nibble)) with next_nibble by word.
+    iFrame "Hown_child".
+    iIntros "Hown_child".
+
+    unfold ht_load_ret.
+    iEval (unfold childP) in "Hchild".
+
+    destruct (decide (nodeptr = null)).
+    {
+      iMod "Hmask" as "_".
+
+      iMod (fupd_mask_subseteq ht_au_mask) as "Hclose_au_mask".
+      {
+        unfold ht_au_mask.
+        apply subseteq_difference_l.
+        set_solver.
+      }
+
+      iMod "Hau" as (m) "[Hown Hclose_au]". (* linearization point *)
+      iDestruct (ghost_var_agree with "Huser_map Hown") as %meq.
+      subst m.
+
+      iDestruct (own_path_lookup _ _ _ h with "Hchild") as "[Hptsto Hptsto_close]"; [exact Hdom|].
+      (* iDestruct (big_sepL_elem_of_acc with "Hchild") as "[Hptsto Hptsto_close]". *)
+      (* { exact Hdom. } *)
+      iDestruct (map_valid with "Hauth_map Hptsto") as %Hlookup.
+      iDestruct ("Hptsto_close" with "Hptsto") as "Hchild".
+
+      iDestruct ("Hchildren_close" with "[Hown_child Hchild]") as "Hchildren".
+      { iExists nodeptr. iFrame. unfold childP.
+        destruct (decide (nodeptr = null)).
+        - iFrame.
+        - contradiction n0.
+      }
+
+      iMod ("Hclose_au" with "Hown") as "HΦ".
+      iMod "Hclose_au_mask" as "_".
+      iMod ("Hclose_ind" with "Hchildren") as "_".
+      iMod ("Hclose_ht" with "[$Hauth_map $Hown_root $Hroot_indirect $Huser_map //]") as "_".
+
+      iApply fupd_mask_intro.
+      { set_solver. }
+      iIntros "_".
+
+      wp_apply wp_interface_type_assert.
+      { auto. }
+
+      wp_bind.
+      replace (bool_decide (nodeptr = null)) with true.
+      2: { symmetry. rewrite (bool_decide_eq_true (nodeptr = null)). exact e. }
+
+      wp_auto.
+      wp_bind.
+      wp_alloc d_ptr as "d_ptr".
+      wp_auto.
+      wp_for_post.
+
+      have Hnone : (user_map !! key = None).
+      {
+        subst user_map.
+        unfold empty_map_fn in Hlookup.
+        have Hflat : flatten hm !! key = (∅ : gmap K V) !! key.
+        { apply (Hbuckets h ∅ key); [exact Hlookup|reflexivity]. }
+        rewrite Hflat.
+        rewrite lookup_empty.
+        done.
+      }
+      iEval (rewrite Hnone; simpl) in "HΦ".
+      iApply "HΦ".
+    }
+
+    iDestruct "Hchild" as (is_entry) "(#Hnodeis_entry & #Hchild)".
+    destruct is_entry.
+    {
+      iDestruct "Hchild" as (ent) "(%Hent_notnull & #Hent & #Hind_null & #Hentry)".
+      iMod "Hmask" as "_".
+
+      (* iEval (rewrite entry_unfold /entry_F) in "Hentry". *)
+      (* iNamed "Hentry". *)
+
+      (* iInv "Hentry_inv" as "HEI" "Hclose_entry". *)
+      (* iEval (unfold entry_inv) in "HEI". *)
+      (* iDestruct "HEI" as "(>? & HEI)". *)
+
+      iMod (fupd_mask_subseteq ht_au_mask) as "Hclose_au_mask".
+      {
+        unfold ht_au_mask.
+        apply subseteq_difference_l.
+        set_solver.
+      }
+
+      iDestruct ("Hchildren_close" with "[Hown_child]") as "Hchildren".
+      {
+        iExists nodeptr. iFrame. unfold childP.
+        destruct (decide (nodeptr = null)).
+        - contradiction n0.
+        - iExists true. iFrame "#". done.
+      }
+
+      iMod "Hclose_au_mask" as "_".
+      iMod ("Hclose_ind" with "[$Hchildren]") as "_".
+      iMod ("Hclose_ht" with "[$Hauth_map $Hown_root $Hroot_indirect $Huser_map //]") as "_".
+
+      iApply fupd_mask_intro.
+      { set_solver. }
+      iIntros "_".
+
+      wp_apply wp_interface_type_assert.
+      { auto. }
+      replace (bool_decide (nodeptr = null)) with false.
+      2: { symmetry. rewrite (bool_decide_eq_false (nodeptr = null)). exact n0. }
+
+      wp_auto.
+
+      wp_apply (wp_node__entry with "[# $]").
+      wp_apply wp_entry__lookup.
+      iFrame "#".
+      rewrite /named.
+      repeat iSplit; eauto.
+      (* { *)
+      (*   rewrite entry_unfold /entry_F. *)
+      (*   iFrame "#". *)
+      (* } *)
+      iAuIntro.
+      iApply aupd_aacc in "Hau".
+      iRevert "Hau".
+      iApply atomic_acc_wand.
+      iSplit.
+      - iIntros.
+        iFrame.
+      - iIntros (m) "HΦ".
+        wp_pures.
+        wp_for_post.
+        iFrame.
+    }
+    iDestruct "Hchild" as (ind) "(%Hnext_path_len & #Hent_null & #Hind & #Hindirect)".
+
+    iDestruct ("Hchildren_close" with "[Hown_child]") as "Hchildren".
+    { iExists nodeptr. iFrame. unfold childP.
+      destruct (decide (nodeptr = null)).
+      - contradiction n0.
+      - iExists false. iFrame "#".
+        iPureIntro. exact Hnext_path_len.
+    }
+
+    iMod "Hmask" as "_".
+    iMod ("Hclose_ind" with "Hchildren") as "_".
+    iMod ("Hclose_ht" with "[$Hauth_map $Hown_root $Hroot_indirect $Huser_map //]") as "_".
+
+    iApply fupd_mask_intro.
+    { set_solver. }
+    iIntros "_".
+
+    wp_apply wp_interface_type_assert.
+    { auto. }
+
+    replace (bool_decide (nodeptr = null)) with false.
+    2: { symmetry. rewrite (bool_decide_eq_false (nodeptr = null)). exact n0. }
+
+    wp_auto.
+    wp_apply (wp_node__indirect with "[$]").
+    wp_for_post.
+    iFrame.
+    iFrame "#".
+    iPureIntro.
+
+    set next := Z.of_nat (sint.nat next_nibble).
+    set next_path := (path ++ [next]).
+
+    have Hlen : length next_path = (length path + 1)%nat by
+                                     rewrite app_length /=.
+
+    have Hz : uint.Z next_nibble = Z.land (h ≫ (sh path - 4)) 15.
+    {
+      rewrite next_nibble_eq.
+      - reflexivity.
+      - auto.
+    }
+
+    split_and!; auto.
+    - rewrite sh_snoc. unfold sh. word.
+    - apply (next_nibble_extend path h next); try done.
+      + unfold h.
+        pose proof (word.unsigned_range (hash_key key)) as [H0 _].
+        exact H0.
+      + unfold next.
+        rewrite Z2Nat.id; [|word].
+        rewrite <- Z2Nat.id with (n:=sint.Z next_nibble) by word.
+        word.
+  Qed.
+
+End proof.
